HybridVerifVecs/MKA/mka_examples.thy
@@ -13,82 +13,62 @@ theory mka_examples
 
 begin
 
-text\<open> Preliminary preparation for the examples.\<close>
+text \<open> Preliminary preparation for the examples.\<close>
 
 no_notation Archimedean_Field.ceiling ("\<lceil>_\<rceil>")
         and Archimedean_Field.floor_ceiling_class.floor ("\<lfloor>_\<rfloor>")
 
-lemma two_eq_zero: "(2::2) = 0" 
-  by simp
 
-lemma four_eq_zero: "(4::4) = 0"
-  by simp
-
-lemma UNIV_2: "(UNIV::2 set) = {0, 1}"
-  apply safe using exhaust_2 two_eq_zero by auto
-
-lemma UNIV_3: "(UNIV::3 set) = {0, 1, 2}"
-  apply safe using exhaust_3 three_eq_zero by auto
-
-lemma UNIV_4: "(UNIV::4 set) = {0, 1, 2, 3}"
-  apply safe using exhaust_4 four_eq_zero by auto
-
-lemma sum_axis_UNIV_3[simp]: "(\<Sum>j\<in>(UNIV::3 set). axis i 1 $ j \<cdot> f j) = (f::3 \<Rightarrow> real) i"
-  unfolding axis_def UNIV_3 apply simp
-  using exhaust_3 by force
-
-
-subsubsection \<open>Pendulum\<close>
+subsubsection\<open>Pendulum\<close>
 
 text \<open> The ODEs @{text "x' t = y t"} and {text "y' t = - x t"} describe the circular motion of 
-a mass attached to a string looked from above. We use @{text "s$0"} to represent the x-coordinate
-and @{text "s$1"} for the y-coordinate. We prove that this motion remains circular. \<close>
-
-\<comment> \<open>Verified with differential invariants. \<close>
+a mass attached to a string looked from above. We use @{text "s$1"} to represent the x-coordinate
+and @{text "s$2"} for the y-coordinate. We prove that this motion remains circular. \<close>
 
 abbreviation fpend :: "real^2 \<Rightarrow> real^2" ("f")
-  where "f s \<equiv> (\<chi> i. if i=0 then s$1 else -s $ 0)"
-
-lemma pendulum_inv:
-  "\<lceil>\<lambda>s. r\<^sup>2 = (s $ 0)\<^sup>2 + (s $ 1)\<^sup>2\<rceil> \<le> wp (x\<acute>= f & G) \<lceil>\<lambda>s. r\<^sup>2 = (s $ 0)\<^sup>2 + (s $ 1)\<^sup>2\<rceil>"
-  by (auto intro!: poly_derivatives diff_invariant_rules)
-
-\<comment> \<open>Verified with the flow. \<close>
+  where "f s \<equiv> (\<chi> i. if i = 1 then s$2 else -s$1)"
 
 abbreviation pend_flow :: "real \<Rightarrow> real^2 \<Rightarrow> real^2" ("\<phi>")
-  where "\<phi> t s \<equiv> (\<chi> i. if i = 0 then s $ 0 \<cdot> cos t + s $ 1 \<cdot> sin t 
-  else - s $ 0 \<cdot> sin t + s $ 1 \<cdot> cos t)"
-
-lemma local_flow_pend: "local_flow f UNIV UNIV \<phi>"
-  apply(unfold_locales, simp_all add: local_lipschitz_def lipschitz_on_def vec_eq_iff, clarsimp)
-  apply(rule_tac x="1" in exI, clarsimp, rule_tac x=1 in exI)
-  apply(simp add: dist_norm norm_vec_def L2_set_def power2_commute UNIV_2)
-   apply(clarify, case_tac "i = 0", simp)
-  using exhaust_2 two_eq_zero by (force intro!: poly_derivatives)+
-
-lemma pendulum_flow:
-  "\<lceil>\<lambda>s. r\<^sup>2 = (s $ 0)\<^sup>2 + (s $ 1)\<^sup>2\<rceil> \<le> wp (x\<acute>= f & G) \<lceil>\<lambda>s. r\<^sup>2 = (s $ 0)\<^sup>2 + (s $ 1)\<^sup>2\<rceil>"
-  by (simp add: local_flow.wp_g_ode[OF local_flow_pend])
+  where "\<phi> t s \<equiv> (\<chi> i. if i = 1 then s$1 * cos t + s$2 * sin t 
+  else - s$1 * sin t + s$2 * cos t)"
 
 \<comment> \<open>Verified by providing dynamics. \<close>
 
 lemma pendulum_dyn:
-  "\<lceil>\<lambda>s. r\<^sup>2 = (s $ 0)\<^sup>2 + (s $ 1)\<^sup>2\<rceil> \<le> wp (EVOL \<phi> G T) \<lceil>\<lambda>s. r\<^sup>2 = (s $ 0)\<^sup>2 + (s $ 1)\<^sup>2\<rceil>"
+  "\<lceil>\<lambda>s. r\<^sup>2 = (s$1)\<^sup>2 + (s$2)\<^sup>2\<rceil> \<le> wp (EVOL \<phi> G T) \<lceil>\<lambda>s. r\<^sup>2 = (s$1)\<^sup>2 + (s$2)\<^sup>2\<rceil>"
   by simp
+
+\<comment> \<open>Verified with differential invariants. \<close>
+
+lemma pendulum_inv:
+  "\<lceil>\<lambda>s. r\<^sup>2 = (s$1)\<^sup>2 + (s$2)\<^sup>2\<rceil> \<le> wp (x\<acute>= f & G) \<lceil>\<lambda>s. r\<^sup>2 = (s$1)\<^sup>2 + (s$2)\<^sup>2\<rceil>"
+  by (auto intro!: poly_derivatives diff_invariant_rules)
+
+\<comment> \<open>Verified with the flow. \<close>
+
+lemma local_flow_pend: "local_flow f UNIV UNIV \<phi>"
+  apply(unfold_locales, simp_all add: local_lipschitz_def lipschitz_on_def vec_eq_iff, clarsimp)
+    apply(rule_tac x="1" in exI, clarsimp, rule_tac x=1 in exI)
+    apply(simp add: dist_norm norm_vec_def L2_set_def power2_commute UNIV_2)
+  by (auto simp: forall_2 intro!: poly_derivatives)
+
+lemma pendulum_flow:
+  "\<lceil>\<lambda>s. r\<^sup>2 = (s$1)\<^sup>2 + (s$2)\<^sup>2\<rceil> \<le> wp (x\<acute>= f & G) \<lceil>\<lambda>s. r\<^sup>2 = (s$1)\<^sup>2 + (s$2)\<^sup>2\<rceil>"
+  by (simp add: local_flow.wp_g_ode[OF local_flow_pend])
 
 \<comment> \<open>Verified as a linear system (using uniqueness). \<close>
 
 abbreviation pend_sq_mtx :: "2 sq_mtx" ("A")
-  where "A \<equiv> sq_mtx_chi (\<chi> i. if i=0 then \<e> 1 else - \<e> 0)"
+  where "A \<equiv> sq_mtx_chi (\<chi> i. if i=1 then \<e> 2 else - \<e> 1)"
 
 lemma pend_sq_mtx_exp_eq_flow: "exp (t *\<^sub>R A) *\<^sub>V s = \<phi> t s"
   apply(rule local_flow.eq_solution[OF local_flow_exp, symmetric])
     apply(rule ivp_solsI, simp add: sq_mtx_vec_prod_def matrix_vector_mult_def)
       apply(force intro!: poly_derivatives simp: matrix_vector_mult_def)
-  using exhaust_2 two_eq_zero by (force simp: vec_eq_iff, auto)
+  using exhaust_2 by (force simp: vec_eq_iff, auto)
 
 lemma pendulum_sq_mtx:
-  "\<lceil>\<lambda>s. r\<^sup>2 = (s$0)\<^sup>2 + (s$1)\<^sup>2\<rceil> \<le> wp (x\<acute>= ((*\<^sub>V) A) & G) \<lceil>\<lambda>s. r\<^sup>2 = (s$0)\<^sup>2 + (s$1)\<^sup>2\<rceil>"
+  "\<lceil>\<lambda>s. r\<^sup>2 = (s$1)\<^sup>2 + (s$2)\<^sup>2\<rceil> \<le> wp (x\<acute>= ((*\<^sub>V) A) & G) \<lceil>\<lambda>s. r\<^sup>2 = (s$1)\<^sup>2 + (s$2)\<^sup>2\<rceil>"
   unfolding local_flow.wp_g_ode[OF local_flow_exp] pend_sq_mtx_exp_eq_flow by auto
 
 no_notation fpend ("f")
@@ -101,96 +81,82 @@ subsubsection\<open> Bouncing Ball \<close>
 text \<open> A ball is dropped from rest at an initial height @{text "h"}. The motion is described with 
 the free-fall equations @{text "x' t = v t"} and @{text "v' t = g"} where @{text "g"} is the 
 constant acceleration due to gravity. The bounce is modelled with a variable assigntment that 
-flips the velocity, thus it is a completely elastic collision with the ground. We use @{text "s$0"} 
-to ball's height and @{text "s$1"} for its velocity. We prove that the ball remains above ground
+flips the velocity, thus it is a completely elastic collision with the ground. We use @{text "s$1"} 
+to ball's height and @{text "s$2"} for its velocity. We prove that the ball remains above ground
 and below its initial resting position. \<close>
+
+abbreviation fball :: "real \<Rightarrow> real^2 \<Rightarrow> real^2" ("f") 
+  where "f g s \<equiv> (\<chi> i. if i = 1 then s$2 else g)"
+
+abbreviation ball_flow :: "real \<Rightarrow> real \<Rightarrow> real^2 \<Rightarrow> real^2" ("\<phi>") 
+  where "\<phi> g t s \<equiv> (\<chi> i. if i = 1 then g * t ^ 2/2 + s$2 * t + s$1 else g * t + s$2)"
 
 \<comment> \<open>Verified with differential invariants. \<close>
 
 named_theorems bb_real_arith "real arithmetic properties for the bouncing ball."
 
-lemma [bb_real_arith]: 
-  assumes "0 > g" and inv: "2 \<cdot> g \<cdot> x - 2 \<cdot> g \<cdot> h = v \<cdot> v"
+lemma inv_imp_pos_le[bb_real_arith]: 
+  assumes "0 > g" and inv: "2 * g * x - 2 * g * h = v * v"
   shows "(x::real) \<le> h"
 proof-
-  have "v \<cdot> v = 2 \<cdot> g \<cdot> x - 2 \<cdot> g \<cdot> h \<and> 0 > g" 
+  have "v * v = 2 * g * x - 2 * g * h \<and> 0 > g" 
     using inv and \<open>0 > g\<close> by auto
-  hence obs:"v \<cdot> v = 2 \<cdot> g \<cdot> (x - h) \<and> 0 > g \<and> v \<cdot> v \<ge> 0" 
+  hence obs:"v * v = 2 * g * (x - h) \<and> 0 > g \<and> v * v \<ge> 0" 
     using left_diff_distrib mult.commute by (metis zero_le_square) 
-  hence "(v \<cdot> v)/(2 \<cdot> g) = (x - h)" 
+  hence "(v * v)/(2 * g) = (x - h)" 
     by auto 
-  also from obs have "(v \<cdot> v)/(2 \<cdot> g) \<le> 0"
+  also from obs have "(v * v)/(2 * g) \<le> 0"
     using divide_nonneg_neg by fastforce 
   ultimately have "h - x \<ge> 0" 
     by linarith
   thus ?thesis by auto
 qed
 
-abbreviation fball :: "real \<Rightarrow> real^2 \<Rightarrow> real^2" ("f") 
-  where "f g s \<equiv> (\<chi> i. if i=(0) then s $ 1 else g)"
-
 lemma bouncing_ball_inv:
   fixes h::real 
-  shows "g < 0 \<Longrightarrow> h \<ge> 0 \<Longrightarrow> \<lceil>\<lambda>s. s $ 0 = h \<and> s $ 1 = 0\<rceil> \<le> 
+  shows "g < 0 \<Longrightarrow> h \<ge> 0 \<Longrightarrow> \<lceil>\<lambda>s. s$1 = h \<and> s$2 = 0\<rceil> \<le> 
   wp 
     (LOOP 
-      ((x\<acute>= f g & (\<lambda> s. s $ 0 \<ge> 0) DINV (\<lambda>s. 2 \<cdot> g \<cdot> s $ 0 - 2 \<cdot> g \<cdot> h - s $ 1 \<cdot> s $ 1 = 0));
-       (IF (\<lambda> s. s $ 0 = 0) THEN (1 ::= (\<lambda>s. - s $ 1)) ELSE skip)) 
-    INV (\<lambda>s. 0 \<le> s $ 0 \<and> 2 \<cdot> g \<cdot> s $ 0 - 2 \<cdot> g \<cdot> h - s $ 1 \<cdot> s $ 1 = 0)
-  ) \<lceil>\<lambda>s. 0 \<le> s $ 0 \<and> s $ 0 \<le> h\<rceil>"
-  apply(rule wp_loopI, simp_all)
-   apply(force simp: bb_real_arith)
-  apply(rule wp_g_odei)
-  by(auto intro!: poly_derivatives diff_invariant_rules)
+      ((x\<acute>= f g & (\<lambda> s. s$1 \<ge> 0) DINV (\<lambda>s. 2 * g * s$1 - 2 * g * h - s$2 * s$2 = 0));
+       (IF (\<lambda> s. s$1 = 0) THEN (2 ::= (\<lambda>s. - s$2)) ELSE skip)) 
+    INV (\<lambda>s. 0 \<le> s$1 \<and> 2 * g * s$1 - 2 * g * h - s$2 * s$2 = 0)
+  ) \<lceil>\<lambda>s. 0 \<le> s$1 \<and> s$1 \<le> h\<rceil>"
+  apply(rule wp_loopI, simp_all, force simp: bb_real_arith)
+  by (rule wp_g_odei) (auto intro!: poly_derivatives diff_invariant_rules)
 
-\<comment> \<open>Verified with the flow. \<close>
+\<comment> \<open>Verified by providing dynamics. \<close>
 
-abbreviation ball_flow :: "real \<Rightarrow> real \<Rightarrow> real^2 \<Rightarrow> real^2" ("\<phi>") 
-  where "\<phi> g t s \<equiv> (\<chi> i. if i=0 then g \<cdot> t ^ 2/2 + s $ 1 \<cdot> t + s $ 0 else g \<cdot> t + s $ 1)"
-
-lemma local_flow_ball: "local_flow (f g) UNIV UNIV (\<phi> g)"
-  apply(unfold_locales, simp_all add: local_lipschitz_def lipschitz_on_def vec_eq_iff, clarsimp)
-  apply(rule_tac x="1/2" in exI, clarsimp, rule_tac x=1 in exI)
-  apply(simp add: dist_norm norm_vec_def L2_set_def UNIV_2)
-   apply(clarsimp, case_tac "i = 0")
-  using exhaust_2 two_eq_zero by (auto intro!: poly_derivatives) force
-
-lemma [bb_real_arith]:
-  assumes invar: "2 \<cdot> g \<cdot> x = 2 \<cdot> g \<cdot> h + v \<cdot> v"
-    and pos: "g \<cdot> \<tau>\<^sup>2 / 2 + v \<cdot> \<tau> + (x::real) = 0"
-  shows "2 \<cdot> g \<cdot> h + (- (g \<cdot> \<tau>) - v) \<cdot> (- (g \<cdot> \<tau>) - v) = 0"
-    and "2 \<cdot> g \<cdot> h + (g \<cdot> \<tau> \<cdot> (g \<cdot> \<tau> + v) + v \<cdot> (g \<cdot> \<tau> + v)) = 0"
+lemma inv_conserv_at_ground[bb_real_arith]:
+  assumes invar: "2 * g * x = 2 * g * h + v * v"
+    and pos: "g * \<tau>\<^sup>2 / 2 + v * \<tau> + (x::real) = 0"
+  shows "2 * g * h + (g * \<tau> * (g * \<tau> + v) + v * (g * \<tau> + v)) = 0"
 proof-
-  from pos have "g \<cdot> \<tau>\<^sup>2  + 2 \<cdot> v \<cdot> \<tau> + 2 \<cdot> x = 0" by auto
-  then have "g\<^sup>2  \<cdot> \<tau>\<^sup>2  + 2 \<cdot> g \<cdot> v \<cdot> \<tau> + 2 \<cdot> g \<cdot> x = 0"
+  from pos have "g * \<tau>\<^sup>2  + 2 * v * \<tau> + 2 * x = 0" by auto
+  then have "g\<^sup>2 * \<tau>\<^sup>2  + 2 * g * v * \<tau> + 2 * g * x = 0"
     by (metis (mono_tags, hide_lams) Groups.mult_ac(1,3) mult_zero_right
         monoid_mult_class.power2_eq_square semiring_class.distrib_left)
-  hence "g\<^sup>2 \<cdot> \<tau>\<^sup>2 + 2 \<cdot> g \<cdot> v \<cdot> \<tau> + v\<^sup>2 + 2 \<cdot> g \<cdot> h = 0"
+  hence "g\<^sup>2 * \<tau>\<^sup>2 + 2 * g * v * \<tau> + v\<^sup>2 + 2 * g * h = 0"
     using invar by (simp add: monoid_mult_class.power2_eq_square) 
-  hence obs: "(g \<cdot> \<tau> + v)\<^sup>2 + 2 \<cdot> g \<cdot> h = 0"
+  hence obs: "(g * \<tau> + v)\<^sup>2 + 2 * g * h = 0"
     apply(subst power2_sum) by (metis (no_types, hide_lams) Groups.add_ac(2, 3) 
         Groups.mult_ac(2, 3) monoid_mult_class.power2_eq_square nat_distrib(2))
-  thus "2 \<cdot> g \<cdot> h + (g \<cdot> \<tau> \<cdot> (g \<cdot> \<tau> + v) + v \<cdot> (g \<cdot> \<tau> + v)) = 0"
-    by (simp add: monoid_mult_class.power2_eq_square)
-  have  "2 \<cdot> g \<cdot> h + (- ((g \<cdot> \<tau>) + v))\<^sup>2 = 0"
-    using obs by (metis Groups.add_ac(2) power2_minus)
-  thus "2 \<cdot> g \<cdot> h + (- (g \<cdot> \<tau>) - v) \<cdot> (- (g \<cdot> \<tau>) - v) = 0"
+  thus "2 * g * h + (g * \<tau> * (g * \<tau> + v) + v * (g * \<tau> + v)) = 0"
     by (simp add: monoid_mult_class.power2_eq_square)
 qed
 
-lemma [bb_real_arith]:
-  assumes invar: "2 \<cdot> g \<cdot> x = 2 \<cdot> g \<cdot> h + v \<cdot> v"
-  shows "2 \<cdot> g \<cdot> (g \<cdot> \<tau>\<^sup>2 / 2 + v \<cdot> \<tau> + (x::real)) = 
-  2 \<cdot> g \<cdot> h + (g \<cdot> \<tau> \<cdot> (g \<cdot> \<tau> + v) + v \<cdot> (g \<cdot> \<tau> + v))" (is "?lhs = ?rhs")
+lemma inv_conserv_at_air[bb_real_arith]:
+  assumes invar: "2 * g * x = 2 * g * h + v * v"
+  shows "2 * g * (g * \<tau>\<^sup>2 / 2 + v * \<tau> + (x::real)) = 
+  2 * g * h + (g * \<tau> * (g * \<tau> + v) + v * (g * \<tau> + v))" (is "?lhs = ?rhs")
 proof-
-  have "?lhs = g\<^sup>2 \<cdot> \<tau>\<^sup>2 + 2 \<cdot> g \<cdot> v \<cdot> \<tau> + 2 \<cdot> g \<cdot> x" 
-      apply(subst Rat.sign_simps(18))+ 
-      by(auto simp: semiring_normalization_rules(29))
-    also have "... = g\<^sup>2 \<cdot> \<tau>\<^sup>2 + 2 \<cdot> g \<cdot> v \<cdot> \<tau> + 2 \<cdot> g \<cdot> h + v \<cdot> v" (is "... = ?middle")
-      by(subst invar, simp)
-    finally have "?lhs = ?middle".
+  have "?lhs = g\<^sup>2 * \<tau>\<^sup>2 + 2 * g * v * \<tau> + 2 * g * x" 
+    apply(subst Rat.sign_simps(18))+ 
+    by(auto simp: semiring_normalization_rules(29))
+  also have "... = g\<^sup>2 * \<tau>\<^sup>2 + 2 * g * v * \<tau> + 2 * g * h + v * v" (is "... = ?middle")
+    by(subst invar, simp)
+  finally have "?lhs = ?middle".
   moreover 
-  {have "?rhs = g \<cdot> g \<cdot> (\<tau> \<cdot> \<tau>) + 2 \<cdot> g \<cdot> v \<cdot> \<tau> + 2 \<cdot> g \<cdot> h + v \<cdot> v"
+  {have "?rhs = g * g * (\<tau> * \<tau>) + 2 * g * v * \<tau> + 2 * g * h + v * v"
     by (simp add: Groups.mult_ac(2,3) semiring_class.distrib_left)
   also have "... = ?middle"
     by (simp add: semiring_normalization_rules(29))
@@ -198,39 +164,45 @@ proof-
   ultimately show ?thesis by auto
 qed
 
-lemma bouncing_ball:
-  fixes h::real 
-  assumes "g < 0" and "h \<ge> 0"
-  shows "g < 0 \<Longrightarrow> h \<ge> 0 \<Longrightarrow> 
-  \<lceil>\<lambda>s. s $ 0 = h \<and> s $ 1 = 0\<rceil> \<le> wp 
-    (LOOP 
-      ((x\<acute>= f g & (\<lambda> s. s $ 0 \<ge> 0));
-      (IF (\<lambda> s. s $ 0 = 0) THEN (1 ::= (\<lambda>s. - s $ 1)) ELSE skip)) 
-    INV (\<lambda>s. 0 \<le> s $ 0 \<and> 2 \<cdot> g \<cdot> s $ 0 = 2 \<cdot> g \<cdot> h + s $ 1 \<cdot> s $ 1)) 
-  \<lceil>\<lambda>s. 0 \<le> s $ 0 \<and> s $ 0 \<le> h\<rceil>"
-  apply(rule wp_loopI, simp_all add: local_flow.wp_g_ode[OF local_flow_ball])
-  by (auto simp: bb_real_arith)
-
-\<comment> \<open>Verified by providing dynamics. \<close>
-
 lemma bouncing_ball_dyn:
   fixes h::real 
   assumes "g < 0" and "h \<ge> 0"
   shows "g < 0 \<Longrightarrow> h \<ge> 0 \<Longrightarrow> 
-  \<lceil>\<lambda>s. s $ 0 = h \<and> s $ 1 = 0\<rceil> \<le> wp 
+  \<lceil>\<lambda>s. s$1 = h \<and> s$2 = 0\<rceil> \<le> wp 
     (LOOP 
-      ((EVOL (\<phi> g) (\<lambda>s. 0 \<le> s $ 0) T);
-      (IF (\<lambda> s. s $ 0 = 0) THEN (1 ::= (\<lambda>s. - s $ 1)) ELSE skip)) 
-    INV (\<lambda>s. 0 \<le> s $ 0 \<and> 2 \<cdot> g \<cdot> s $ 0 = 2 \<cdot> g \<cdot> h + s $ 1 \<cdot> s $ 1)) 
-  \<lceil>\<lambda>s. 0 \<le> s $ 0 \<and> s $ 0 \<le> h\<rceil>"
+      ((EVOL (\<phi> g) (\<lambda>s. 0 \<le> s$1) T);
+      (IF (\<lambda> s. s$1 = 0) THEN (2 ::= (\<lambda>s. - s$2)) ELSE skip)) 
+    INV (\<lambda>s. 0 \<le> s$1 \<and> 2 * g * s$1 = 2 * g * h + s$2 * s$2)) 
+  \<lceil>\<lambda>s. 0 \<le> s$1 \<and> s$1 \<le> h\<rceil>"
   by (rule wp_loopI) (auto simp: bb_real_arith)
+
+\<comment> \<open>Verified with the flow. \<close>
+
+lemma local_flow_ball: "local_flow (f g) UNIV UNIV (\<phi> g)"
+  apply(unfold_locales, simp_all add: local_lipschitz_def lipschitz_on_def vec_eq_iff, clarsimp)
+    apply(rule_tac x="1/2" in exI, clarsimp, rule_tac x=1 in exI)
+    apply(simp add: dist_norm norm_vec_def L2_set_def UNIV_2)
+  by (auto simp: forall_2 intro!: poly_derivatives)
+
+lemma bouncing_ball_flow:
+  fixes h::real 
+  assumes "g < 0" and "h \<ge> 0"
+  shows "g < 0 \<Longrightarrow> h \<ge> 0 \<Longrightarrow> 
+  \<lceil>\<lambda>s. s$1 = h \<and> s$2 = 0\<rceil> \<le> wp 
+    (LOOP 
+      ((x\<acute>= f g & (\<lambda> s. s$1 \<ge> 0));
+      (IF (\<lambda> s. s$1 = 0) THEN (2 ::= (\<lambda>s. - s$2)) ELSE skip)) 
+    INV (\<lambda>s. 0 \<le> s$1 \<and> 2 * g * s$1 = 2 * g * h + s$2 * s$2)) 
+  \<lceil>\<lambda>s. 0 \<le> s$1 \<and> s$1 \<le> h\<rceil>"
+  apply(rule wp_loopI, simp_all add: local_flow.wp_g_ode[OF local_flow_ball])
+  by (auto simp: bb_real_arith)
 
 \<comment> \<open>Verified as a linear system (computing exponential). \<close>
 
 abbreviation ball_sq_mtx :: "3 sq_mtx" ("A")
-  where "ball_sq_mtx \<equiv> sq_mtx_chi (\<chi> i. if i=0 then \<e> 1 else if i=1 then \<e> 2 else 0)"
+  where "ball_sq_mtx \<equiv> sq_mtx_chi (\<chi> i. if i = 1 then \<e> 2 else if i = 2 then \<e> 3 else 0)"
 
-lemma ball_sq_mtx_pow2: "A\<^sup>2 = sq_mtx_chi (\<chi> i. if i=0 then \<e> 2 else 0)"
+lemma ball_sq_mtx_pow2: "A\<^sup>2 = sq_mtx_chi (\<chi> i. if i = 1 then \<e> 3 else 0)"
   unfolding monoid_mult_class.power2_eq_square times_sq_mtx_def
   by (simp add: sq_mtx_chi_inject vec_eq_iff matrix_matrix_mult_def)
 
@@ -245,30 +217,31 @@ lemma exp_ball_sq_mtx: "exp (\<tau> *\<^sub>R A) = ((\<tau> *\<^sub>R A)\<^sup>2
   using ball_sq_mtx_powN by (simp_all add: numeral_2_eq_2)
  
 lemma exp_ball_sq_mtx_simps:
-  "exp (\<tau> *\<^sub>R A) $$ 0 $ 0 = 1" "exp (\<tau> *\<^sub>R A) $$ 0 $ 1 = \<tau>" "exp (\<tau> *\<^sub>R A) $$ 0 $ 2 = \<tau>^2/2"
-  "exp (\<tau> *\<^sub>R A) $$ 1 $ 0 = 0" "exp (\<tau> *\<^sub>R A) $$ 1 $ 1 = 1" "exp (\<tau> *\<^sub>R A) $$ 1 $ 2 = \<tau>"
-  "exp (\<tau> *\<^sub>R A) $$ 2 $ 0 = 0" "exp (\<tau> *\<^sub>R A) $$ 2 $ 1 = 0" "exp (\<tau> *\<^sub>R A) $$ 2 $ 2 = 1"
+  "exp (\<tau> *\<^sub>R A) $$ 1 $ 1 = 1" "exp (\<tau> *\<^sub>R A) $$ 1 $ 2 = \<tau>" "exp (\<tau> *\<^sub>R A) $$ 1 $ 3 = \<tau>^2/2"
+  "exp (\<tau> *\<^sub>R A) $$ 2 $ 1 = 0" "exp (\<tau> *\<^sub>R A) $$ 2 $ 2 = 1" "exp (\<tau> *\<^sub>R A) $$ 2 $ 3 = \<tau>"
+  "exp (\<tau> *\<^sub>R A) $$ 3 $ 1 = 0" "exp (\<tau> *\<^sub>R A) $$ 3 $ 2 = 0" "exp (\<tau> *\<^sub>R A) $$ 3 $ 3 = 1"
   unfolding exp_ball_sq_mtx scaleR_power ball_sq_mtx_pow2
   by (auto simp: plus_sq_mtx_def scaleR_sq_mtx_def one_sq_mtx_def 
       mat_def scaleR_vec_def axis_def plus_vec_def)
 
 lemma bouncing_ball_sq_mtx:
-  "\<lceil>\<lambda>s. 0 \<le> s $ 0 \<and> s $ 0 = h \<and> s $ 1 = 0 \<and> 0 > s $ 2\<rceil> \<le> wp 
+  "\<lceil>\<lambda>s. 0 \<le> s$1 \<and> s$1 = h \<and> s$2 = 0 \<and> 0 > s$3\<rceil> \<le> wp 
     (LOOP 
-      ((x\<acute>=(*\<^sub>V)A & (\<lambda> s. s $ 0 \<ge> 0));
-      (IF (\<lambda> s. s $ 0 = 0) THEN (1 ::= (\<lambda>s. - s $ 1)) ELSE skip))
-    INV (\<lambda>s. 0 \<le> s$0 \<and> 0 > s$2 \<and> 2 \<cdot> s$2 \<cdot> s$0 = 2 \<cdot> s$2 \<cdot> h + (s$1 \<cdot> s$1)))
-  \<lceil>\<lambda>s. 0 \<le> s $ 0 \<and> s $ 0 \<le> h\<rceil>"
+      ((x\<acute>=(*\<^sub>V)A & (\<lambda> s. s$1 \<ge> 0));
+      (IF (\<lambda> s. s$1 = 0) THEN (2 ::= (\<lambda>s. - s$2)) ELSE skip))
+    INV (\<lambda>s. 0 \<le> s$1 \<and> 0 > s$3 \<and> 2 \<cdot> s$3 \<cdot> s$1 = 2 \<cdot> s$3 \<cdot> h + (s$2 \<cdot> s$2)))
+  \<lceil>\<lambda>s. 0 \<le> s$1 \<and> s$1 \<le> h\<rceil>"
   apply(rule wp_loopI, simp_all add: local_flow.wp_g_ode[OF local_flow_exp])
    apply(force simp: bb_real_arith)
   apply(simp add: sq_mtx_vec_prod_eq)
   unfolding UNIV_3 apply(simp add: exp_ball_sq_mtx_simps, safe)
-  using bb_real_arith(3) apply(force simp: add.commute mult.commute)
-  using bb_real_arith(4) by (force simp: add.commute mult.commute)
+  using bb_real_arith(2) apply(force simp: add.commute mult.commute)
+  using bb_real_arith(3) by (force simp: add.commute mult.commute)
 
 no_notation fball ("f")
         and ball_flow ("\<phi>")
         and ball_sq_mtx ("A")
+
 
 subsubsection\<open> Thermostat \<close>
 
@@ -276,31 +249,31 @@ text \<open> A thermostat has a chronometer, a thermometer and a switch to turn 
 At most every @{text "t"} minutes, it sets its chronometer to @{term "0::real"}, it registers 
 the room temperature, and it turns the heater on (or off) based on this reading. The temperature 
 follows the ODE @{text "T' = - a * (T - U)"} where @{text "U"} is @{text "L \<ge> 0"} when the heater 
-is on, and @{text "0"} when it is off. We use @{term "0::4"} to denote the room's temperature, 
-@{term "1::4"} is time as measured by the thermostat's chronometer, @{term "2::4"} is the 
-temperature detected by the thermometer, and @{term "3::4"} states whether the heater is on 
-(@{text "s$3 = 1"}) or off (@{text "s$3 = 0"}). We prove that the thermostat keeps the room's 
+is on, and @{text "0"} when it is off. We use @{term "1::4"} to denote the room's temperature, 
+@{term "2::4"} is time as measured by the thermostat's chronometer, @{term "3::4"} is the 
+temperature detected by the thermometer, and @{term "4::4"} states whether the heater is on 
+(@{text "s$4 = 1"}) or off (@{text "s$4 = 0"}). We prove that the thermostat keeps the room's 
 temperature between @{text "Tmin"} and @{text "Tmax"}. \<close>
 
 abbreviation temp_vec_field :: "real \<Rightarrow> real \<Rightarrow> real^4 \<Rightarrow> real^4" ("f")
-  where "f a L s \<equiv> (\<chi> i. if i = 1 then 1 else (if i = 0 then - a * (s$0 - L) else 0))"
+  where "f a L s \<equiv> (\<chi> i. if i = 2 then 1 else (if i = 1 then - a * (s$1 - L) else 0))"
 
 abbreviation temp_flow :: "real \<Rightarrow> real \<Rightarrow> real \<Rightarrow> real^4 \<Rightarrow> real^4" ("\<phi>")
-  where "\<phi> a L t s \<equiv> (\<chi> i. if i = 0 then - exp(-a * t) * (L - s$0) + L else 
-  (if i = 1 then t + s$1 else (if i = 2 then s$2 else s$3)))"
+  where "\<phi> a L t s \<equiv> (\<chi> i. if i = 1 then - exp(-a * t) * (L - s$1) + L else 
+  (if i = 2 then t + s$2 else s$i))"
 
 \<comment> \<open>Verified with the flow. \<close>
 
-lemma norm_diff_temp_dyn: "0 < a \<Longrightarrow> \<parallel>f a L s\<^sub>1 - f a L s\<^sub>2\<parallel> = \<bar>a\<bar> * \<bar>s\<^sub>1$0 - s\<^sub>2$0\<bar>"
+lemma norm_diff_temp_dyn: "0 < a \<Longrightarrow> \<parallel>f a L s\<^sub>1 - f a L s\<^sub>2\<parallel> = \<bar>a\<bar> * \<bar>s\<^sub>1$1 - s\<^sub>2$1\<bar>"
 proof(simp add: norm_vec_def L2_set_def, unfold UNIV_4, simp)
   assume a1: "0 < a"
   have f2: "\<And>r ra. \<bar>(r::real) + - ra\<bar> = \<bar>ra + - r\<bar>"
     by (metis abs_minus_commute minus_real_def)
   have "\<And>r ra rb. (r::real) * ra + - (r * rb) = r * (ra + - rb)"
     by (metis minus_real_def right_diff_distrib)
-  hence "\<bar>a * (s\<^sub>1$0 + - L) + - (a * (s\<^sub>2$0 + - L))\<bar> = a * \<bar>s\<^sub>1$0 + - s\<^sub>2$0\<bar>"
+  hence "\<bar>a * (s\<^sub>1$1 + - L) + - (a * (s\<^sub>2$1 + - L))\<bar> = a * \<bar>s\<^sub>1$1 + - s\<^sub>2$1\<bar>"
     using a1 by (simp add: abs_mult)
-  thus "\<bar>a * (s\<^sub>2$0 - L) - a * (s\<^sub>1$0 - L)\<bar> = a * \<bar>s\<^sub>1$0 - s\<^sub>2$0\<bar>"
+  thus "\<bar>a * (s\<^sub>2$1 - L) - a * (s\<^sub>1$1 - L)\<bar> = a * \<bar>s\<^sub>1$1 - s\<^sub>2$1\<bar>"
     using f2 minus_real_def by presburger
 qed
 
@@ -309,14 +282,13 @@ lemma local_lipschitz_temp_dyn:
   shows "local_lipschitz UNIV UNIV (\<lambda>t::real. f a L)"
   apply(unfold local_lipschitz_def lipschitz_on_def dist_norm)
   apply(clarsimp, rule_tac x=1 in exI, clarsimp, rule_tac x=a in exI)
-  using assms apply(simp_all add: norm_diff_temp_dyn)
+  using assms 
+  apply(simp_all add: norm_diff_temp_dyn)
   apply(simp add: norm_vec_def L2_set_def, unfold UNIV_4, clarsimp)
   unfolding real_sqrt_abs[symmetric] by (rule real_le_lsqrt) auto
 
-
 lemma local_flow_temp: "a > 0 \<Longrightarrow> local_flow (f a L) UNIV UNIV (\<phi> a L)"
-  by (unfold_locales, auto intro!: poly_derivatives local_lipschitz_temp_dyn 
-      simp: forall_4 vec_eq_iff four_eq_zero)
+  by (unfold_locales, auto intro!: poly_derivatives local_lipschitz_temp_dyn simp: forall_4 vec_eq_iff)
 
 lemma temp_dyn_down_real_arith:
   assumes "a > 0" and Thyps: "0 < Tmin" "Tmin \<le> T" "T \<le> Tmax"
@@ -369,17 +341,17 @@ lemmas fbox_temp_dyn = local_flow.fbox_g_ode_ivl[OF local_flow_temp _ UNIV_I]
 
 lemma thermostat: 
   assumes "a > 0" and "0 \<le> t" and "0 < Tmin" and "Tmax < L"
-  shows "\<lceil>\<lambda>s. Tmin \<le> s$0 \<and> s$0 \<le> Tmax \<and> s$3 = 0\<rceil> \<le> wp
+  shows "\<lceil>\<lambda>s. Tmin \<le> s$1 \<and> s$1 \<le> Tmax \<and> s$4 = 0\<rceil> \<le> wp
   (LOOP 
     \<comment> \<open>control\<close>
-    ((1 ::= (\<lambda>s. 0));(2 ::= (\<lambda>s. s$0));
-    (IF (\<lambda>s. s$3 = 0 \<and> s$2 \<le> Tmin + 1) THEN (3 ::= (\<lambda>s.1)) ELSE 
-    (IF (\<lambda>s. s$3 = 1 \<and> s$2 \<ge> Tmax - 1) THEN (3 ::= (\<lambda>s.0)) ELSE skip));
+    ((2 ::= (\<lambda>s. 0));(3 ::= (\<lambda>s. s$1));
+    (IF (\<lambda>s. s$4 = 0 \<and> s$3 \<le> Tmin + 1) THEN (4 ::= (\<lambda>s.1)) ELSE 
+    (IF (\<lambda>s. s$4 = 1 \<and> s$3 \<ge> Tmax - 1) THEN (4 ::= (\<lambda>s.0)) ELSE skip));
     \<comment> \<open>dynamics\<close>
-    (IF (\<lambda>s. s$3 = 0) THEN (x\<acute>=(f a 0) & (\<lambda>s. s$1 \<le> - (ln (Tmin/s$2))/a) on {0..t} UNIV @ 0) 
-    ELSE (x\<acute>=(f a L) & (\<lambda>s. s$1 \<le> - (ln ((L-Tmax)/(L-s$2)))/a) on {0..t} UNIV @ 0)) )
-  INV (\<lambda>s. Tmin \<le>s$0 \<and> s$0 \<le> Tmax \<and> (s$3 = 0 \<or> s$3 = 1)))
-  \<lceil>\<lambda>s. Tmin \<le> s$0 \<and> s$0 \<le> Tmax\<rceil>"
+    (IF (\<lambda>s. s$4 = 0) THEN (x\<acute>=(f a 0) & (\<lambda>s. s$2 \<le> - (ln (Tmin/s$3))/a) on {0..t} UNIV @ 0) 
+    ELSE (x\<acute>=(f a L) & (\<lambda>s. s$2 \<le> - (ln ((L-Tmax)/(L-s$3)))/a) on {0..t} UNIV @ 0)) )
+  INV (\<lambda>s. Tmin \<le>s$1 \<and> s$1 \<le> Tmax \<and> (s$4 = 0 \<or> s$4 = 1)))
+  \<lceil>\<lambda>s. Tmin \<le> s$1 \<and> s$1 \<le> Tmax\<rceil>"
   apply(rule wp_loopI, simp_all add: fbox_temp_dyn[OF assms(1,2)])
   using temp_dyn_up_real_arith[OF assms(1) _ _ assms(4), of Tmin]
     and temp_dyn_down_real_arith[OF assms(1,3), of _ Tmax] by auto
