HybridVerifVecs/KAT/kat2ndfun.thy
@@ -1,0 +1,449 @@
+(*  Title:       Verification and refinement of hybrid systems in the relational KAT
+    Author:      Jonathan Julián Huerta y Munive, 2019
+    Maintainer:  Jonathan Julián Huerta y Munive <jjhuertaymunive1@sheffield.ac.uk>
+*)
+
+section \<open> Verification and refinement of HS in the relational KAT \<close>
+
+text \<open> We use our state transformers model to obtain verification and refinement components for 
+hybrid programs. We devise three methods for reasoning with evolution commands and their continuous 
+dynamics: providing flows, solutions or invariants. \<close>
+
+theory kat2ndfun
+  imports 
+    "../hs_prelims_ka"
+    "../hs_prelims_dyn_sys"
+
+begin
+
+subsection \<open> Store and Hoare triples \<close>
+
+type_synonym 'a pred = "'a \<Rightarrow> bool"
+
+\<comment> \<open>We start by deleting some conflicting notation.\<close>
+
+no_notation Archimedean_Field.ceiling ("\<lceil>_\<rceil>")
+        and Archimedean_Field.floor_ceiling_class.floor ("\<lfloor>_\<rfloor>")
+        and tau ("\<tau>")
+        and Relation.relcomp (infixl ";" 75)
+        and proto_near_quantale_class.bres (infixr "\<rightarrow>" 60)
+
+\<comment> \<open>Canonical lifting from predicates to state transformers and its simplification rules\<close>
+
+definition p2ndf :: "'a pred \<Rightarrow> 'a nd_fun" ("(1\<lceil>_\<rceil>)")
+  where "\<lceil>Q\<rceil> \<equiv> (\<lambda> x::'a. {s::'a. s = x \<and> Q s})\<^sup>\<bullet>"
+
+lemma p2ndf_simps[simp]: 
+  "\<lceil>P\<rceil> \<le> \<lceil>Q\<rceil> = (\<forall>s. P s \<longrightarrow> Q s)"
+  "(\<lceil>P\<rceil> = \<lceil>Q\<rceil>) = (\<forall>s. P s = Q s)"
+  "(\<lceil>P\<rceil> \<cdot> \<lceil>Q\<rceil>) = \<lceil>\<lambda>s. P s \<and> Q s\<rceil>"
+  "(\<lceil>P\<rceil> + \<lceil>Q\<rceil>) = \<lceil>\<lambda>s. P s \<or> Q s\<rceil>"
+  "\<tt>\<tt> \<lceil>P\<rceil> = \<lceil>P\<rceil>"
+  "n \<lceil>P\<rceil> = \<lceil>\<lambda>s. \<not> P s\<rceil>"
+  unfolding p2ndf_def one_nd_fun_def less_eq_nd_fun_def times_nd_fun_def plus_nd_fun_def 
+  by (auto simp: nd_fun_eq_iff kcomp_def le_fun_def n_op_nd_fun_def)
+
+\<comment> \<open> Meaning of the state-transformer Hoare triple \<close>
+
+lemma ndfun_kat_H: "Hoare \<lceil>P\<rceil> X \<lceil>Q\<rceil> \<longleftrightarrow> (\<forall>s s'. P s \<longrightarrow> s' \<in> (X\<^sub>\<bullet>) s \<longrightarrow> Q s')"
+  unfolding Hoare_def p2ndf_def less_eq_nd_fun_def times_nd_fun_def kcomp_def 
+  by (auto simp add: le_fun_def n_op_nd_fun_def)
+
+\<comment> \<open> Hoare triple for skip and a simp-rule \<close>
+
+abbreviation "skip \<equiv> (1::'a nd_fun)"
+
+lemma H_skip: "Hoare \<lceil>P\<rceil> skip \<lceil>P\<rceil>"
+  using H_skip by blast
+
+lemma sH_skip[simp]: "Hoare \<lceil>P\<rceil> skip \<lceil>Q\<rceil> \<longleftrightarrow> \<lceil>P\<rceil> \<le> \<lceil>Q\<rceil>"
+  unfolding ndfun_kat_H by (simp add: one_nd_fun_def)
+
+\<comment> \<open> We introduce assignments and compute derive their rule of Hoare logic. \<close>
+
+definition vec_upd :: "('a^'b) \<Rightarrow> 'b \<Rightarrow> 'a \<Rightarrow> 'a^'b"
+  where "vec_upd s i a = (\<chi> j. ((($) s)(i := a)) j)"
+
+definition assign :: "'b \<Rightarrow> ('a^'b \<Rightarrow> 'a) \<Rightarrow> ('a^'b) nd_fun" ("(2_ ::= _)" [70, 65] 61) 
+  where "(x ::= e) = (\<lambda>s. {vec_upd s x (e s)})\<^sup>\<bullet>"
+
+lemma H_assign: "P = (\<lambda>s. Q (\<chi> j. ((($) s)(x := (e s))) j)) \<Longrightarrow> Hoare \<lceil>P\<rceil> (x ::= e) \<lceil>Q\<rceil>"
+  unfolding ndfun_kat_H assign_def vec_upd_def by force
+
+lemma sH_assign[simp]: "Hoare \<lceil>P\<rceil> (x ::= e) \<lceil>Q\<rceil> \<longleftrightarrow> (\<forall>s. P s \<longrightarrow> Q (\<chi> j. ((($) s)(x := (e s))) j))"
+  unfolding ndfun_kat_H vec_upd_def assign_def by (auto simp: fun_upd_def)
+
+\<comment> \<open> Next, the Hoare rule of the composition \<close>
+
+abbreviation seq_seq :: "'a nd_fun \<Rightarrow> 'a nd_fun \<Rightarrow> 'a nd_fun" (infixl ";" 75)
+  where "f ; g \<equiv> f \<cdot> g"
+
+lemma H_seq: "Hoare \<lceil>P\<rceil> X \<lceil>R\<rceil> \<Longrightarrow> Hoare \<lceil>R\<rceil> Y \<lceil>Q\<rceil> \<Longrightarrow> Hoare \<lceil>P\<rceil> (X ; Y) \<lceil>Q\<rceil>"
+  by (auto intro: H_seq)
+
+lemma sH_seq: "Hoare \<lceil>P\<rceil> (X ; Y) \<lceil>Q\<rceil> = Hoare \<lceil>P\<rceil> (X) \<lceil>\<lambda>s. \<forall>s'. s' \<in> (Y\<^sub>\<bullet>) s \<longrightarrow> Q s'\<rceil>"
+  unfolding ndfun_kat_H by (auto simp: times_nd_fun_def kcomp_def)
+
+\<comment> \<open> Rewriting the Hoare rule for the conditional statement \<close>
+
+abbreviation cond_sugar :: "'a pred \<Rightarrow> 'a nd_fun \<Rightarrow> 'a nd_fun \<Rightarrow> 'a nd_fun" ("IF _ THEN _ ELSE _" [64,64] 63) 
+  where "IF B THEN X ELSE Y \<equiv> kat_cond \<lceil>B\<rceil> X Y"
+
+lemma H_cond: "Hoare \<lceil>\<lambda>s. P s \<and> B s\<rceil> X \<lceil>Q\<rceil> \<Longrightarrow> Hoare \<lceil>\<lambda>s. P s \<and> \<not> B s\<rceil> Y \<lceil>Q\<rceil> \<Longrightarrow> 
+  Hoare \<lceil>P\<rceil> (IF B THEN X ELSE Y) \<lceil>Q\<rceil>"
+  by (rule H_cond, simp_all)
+
+lemma sH_cond[simp]: "Hoare \<lceil>P\<rceil> (IF B THEN X ELSE Y) \<lceil>Q\<rceil> \<longleftrightarrow> 
+  (Hoare \<lceil>\<lambda>s. P s \<and> B s\<rceil> X \<lceil>Q\<rceil> \<and> Hoare \<lceil>\<lambda>s. P s \<and> \<not> B s\<rceil> Y \<lceil>Q\<rceil>)"
+  by (auto simp: H_cond_iff ndfun_kat_H)
+
+\<comment> \<open> Rewriting the Hoare rule for the while loop \<close>
+
+abbreviation while_inv_sugar :: "'a pred \<Rightarrow> 'a pred \<Rightarrow> 'a nd_fun \<Rightarrow> 'a nd_fun" ("WHILE _ INV _ DO _" [64,64,64] 63) 
+  where "WHILE B INV I DO X \<equiv> kat_while_inv \<lceil>B\<rceil> \<lceil>I\<rceil> X"
+
+lemma sH_while_inv: "\<forall>s. P s \<longrightarrow> I s \<Longrightarrow> \<forall>s. I s \<and> \<not> B s \<longrightarrow> Q s \<Longrightarrow> Hoare \<lceil>\<lambda>s. I s \<and> B s\<rceil> X \<lceil>I\<rceil> 
+  \<Longrightarrow> Hoare \<lceil>P\<rceil> (WHILE B INV I DO X) \<lceil>Q\<rceil>"
+  by (rule H_while_inv, simp_all add: ndfun_kat_H)
+
+\<comment> \<open> Finally, we add a Hoare triple rule for finite iterations. \<close>
+
+abbreviation loopi_sugar :: "'a nd_fun \<Rightarrow> 'a pred \<Rightarrow> 'a nd_fun" ("LOOP _ INV _ " [64,64] 63)
+  where "LOOP X INV I \<equiv> kat_loop_inv X \<lceil>I\<rceil>"
+
+lemma H_loop: "Hoare \<lceil>P\<rceil> X \<lceil>P\<rceil> \<Longrightarrow> Hoare \<lceil>P\<rceil> (LOOP X INV I) \<lceil>P\<rceil>"
+  by (auto intro: H_loop)
+
+lemma H_loopI: "Hoare \<lceil>I\<rceil> X \<lceil>I\<rceil> \<Longrightarrow> \<lceil>P\<rceil> \<le> \<lceil>I\<rceil> \<Longrightarrow> \<lceil>I\<rceil> \<le> \<lceil>Q\<rceil> \<Longrightarrow> Hoare \<lceil>P\<rceil> (LOOP X INV I) \<lceil>Q\<rceil>"
+  using H_loop_inv[of "\<lceil>P\<rceil>" "\<lceil>I\<rceil>" X "\<lceil>Q\<rceil>"] by auto
+
+
+subsection\<open> Verification of hybrid programs \<close>
+
+\<comment> \<open>Verification by providing evolution\<close>
+
+definition g_evol :: "(('a::ord) \<Rightarrow> 'b \<Rightarrow> 'b) \<Rightarrow> 'b pred \<Rightarrow> 'a set \<Rightarrow> 'b nd_fun" ("EVOL")
+  where "EVOL \<phi> G T = (\<lambda>s. g_orbit (\<lambda>t. \<phi> t s) G T)\<^sup>\<bullet>"
+
+lemma H_g_evol: 
+  fixes \<phi> :: "('a::preorder) \<Rightarrow> 'b \<Rightarrow> 'b"
+  assumes "P = (\<lambda>s. (\<forall>t\<in>T. (\<forall>\<tau>\<in>down T t. G (\<phi> \<tau> s)) \<longrightarrow> Q (\<phi> t s)))"
+  shows "Hoare \<lceil>P\<rceil> (EVOL \<phi> G T) \<lceil>Q\<rceil>"
+  unfolding ndfun_kat_H g_evol_def g_orbit_eq using assms by clarsimp
+
+lemma sH_g_evol[simp]:  
+  fixes \<phi> :: "('a::preorder) \<Rightarrow> 'b \<Rightarrow> 'b"
+  shows "Hoare \<lceil>P\<rceil> (EVOL \<phi> G T) \<lceil>Q\<rceil> = (\<forall>s. P s \<longrightarrow> (\<forall>t\<in>T. (\<forall>\<tau>\<in>down T t. G (\<phi> \<tau> s)) \<longrightarrow> Q (\<phi> t s)))"
+  unfolding ndfun_kat_H g_evol_def g_orbit_eq by auto
+
+\<comment> \<open>Verification by providing solutions\<close>
+
+definition g_ode ::"(('a::banach)\<Rightarrow>'a) \<Rightarrow> 'a pred \<Rightarrow> real set \<Rightarrow> 'a set \<Rightarrow> 
+  real \<Rightarrow> 'a nd_fun" ("(1x\<acute>= _ & _ on _ _ @ _)") 
+  where "(x\<acute>= f & G on T S @ t\<^sub>0) \<equiv> (\<lambda> s. g_orbital f G T S t\<^sub>0 s)\<^sup>\<bullet>"
+
+lemma H_g_orbital: 
+  "P = (\<lambda>s. (\<forall>X\<in>ivp_sols (\<lambda>t. f) T S t\<^sub>0 s. \<forall>t\<in>T. (\<forall>\<tau>\<in>down T t. G (X \<tau>)) \<longrightarrow> Q (X t))) \<Longrightarrow> 
+  Hoare \<lceil>P\<rceil> (x\<acute>= f & G on T S @ t\<^sub>0) \<lceil>Q\<rceil>"
+  unfolding ndfun_kat_H g_ode_def g_orbital_eq by clarsimp
+
+lemma sH_g_orbital: "Hoare \<lceil>P\<rceil> (x\<acute>= f & G on T S @ t\<^sub>0) \<lceil>Q\<rceil> = 
+  (\<forall>s. P s \<longrightarrow> (\<forall>X\<in>ivp_sols (\<lambda>t. f) T S t\<^sub>0 s. \<forall>t\<in>T. (\<forall>\<tau>\<in>down T t. G (X \<tau>)) \<longrightarrow> Q (X t)))"
+  unfolding g_orbital_eq g_ode_def ndfun_kat_H by auto
+
+context local_flow
+begin
+
+lemma H_g_ode:
+  assumes "P = (\<lambda>s. s \<in> S \<longrightarrow> (\<forall>t\<in>T. (\<forall>\<tau>\<in>down T t. G (\<phi> \<tau> s)) \<longrightarrow> Q (\<phi> t s)))" 
+  shows "Hoare \<lceil>P\<rceil> (x\<acute>= f & G on T S @ 0) \<lceil>Q\<rceil>"
+proof(unfold ndfun_kat_H g_ode_def g_orbital_eq assms, clarsimp)
+  fix s t X
+  assume hyps: "t \<in> T" "\<forall>x. x \<in> T \<and> x \<le> t \<longrightarrow> G (X x)" "X \<in> Sols (\<lambda>t. f) T S 0 s"
+     and main: "s \<in> S \<longrightarrow> (\<forall>t\<in>T. (\<forall>\<tau>. \<tau> \<in> T \<and> \<tau> \<le> t \<longrightarrow> G (\<phi> \<tau> s)) \<longrightarrow> Q (\<phi> t s))"
+  have "s \<in> S"
+    using ivp_solsD[OF hyps(3)] init_time by auto
+  hence "\<forall>\<tau>\<in>down T t. X \<tau> = \<phi> \<tau> s"
+    using eq_solution hyps by blast
+  thus "Q (X t)"
+    using main \<open>s \<in> S\<close> hyps by fastforce
+qed
+
+lemma sH_g_ode: "Hoare \<lceil>P\<rceil> (x\<acute>= f & G on T S @ 0) \<lceil>Q\<rceil> = 
+  (\<forall>s\<in>S. P s \<longrightarrow> (\<forall>t\<in>T. (\<forall>\<tau>\<in>down T t. G (\<phi> \<tau> s)) \<longrightarrow> Q (\<phi> t s)))"
+proof(unfold sH_g_orbital, clarsimp, safe)
+  fix s t
+  assume hyps: "s \<in> S" "P s" "t\<in>T" "\<forall>\<tau>. \<tau> \<in> T \<and> \<tau> \<le> t \<longrightarrow> G (\<phi> \<tau> s)"
+    and main: "\<forall>s. P s \<longrightarrow> (\<forall>X\<in>Sols (\<lambda>t. f) T S 0 s. \<forall>t\<in>T. (\<forall>\<tau>. \<tau> \<in> T \<and> \<tau> \<le> t \<longrightarrow> G (X \<tau>)) \<longrightarrow> Q (X t))"
+  hence "(\<lambda>t. \<phi> t s) \<in> Sols (\<lambda>t. f) T S 0 s"
+    using in_ivp_sols by blast
+  thus "Q (\<phi> t s)"
+    using main hyps by fastforce
+next
+  fix s X t
+  assume hyps: "P s" "X \<in> Sols (\<lambda>t. f) T S 0 s" "t \<in> T"  "\<forall>\<tau>. \<tau> \<in> T \<and> \<tau> \<le> t \<longrightarrow> G (X \<tau>)"
+    and main: "\<forall>s\<in>S. P s \<longrightarrow> (\<forall>t\<in>T. (\<forall>\<tau>. \<tau> \<in> T \<and> \<tau> \<le> t \<longrightarrow> G (\<phi> \<tau> s)) \<longrightarrow> Q (\<phi> t s))"
+  hence obs: "s \<in> S"
+    using ivp_sols_def[of "\<lambda>t. f"] init_time by auto
+  hence "\<forall>\<tau>\<in>down T t. X \<tau> = \<phi> \<tau> s"
+    using eq_solution hyps by blast
+  thus "Q (X t)"
+    using hyps main obs by auto
+qed
+
+lemma sH_g_ode_ivl: "\<tau> \<ge> 0 \<Longrightarrow> \<tau> \<in> T \<Longrightarrow> Hoare \<lceil>P\<rceil> (x\<acute>= f & G on {0..\<tau>} S @ 0) \<lceil>Q\<rceil> = 
+  (\<forall>s\<in>S. P s \<longrightarrow> (\<forall>t\<in>{0..\<tau>}. (\<forall>\<tau>\<in>{0..t}. G (\<phi> \<tau> s)) \<longrightarrow> Q (\<phi> t s)))"
+proof(unfold sH_g_orbital, clarsimp, safe)
+  fix s t
+  assume hyps: "0 \<le> \<tau>" "\<tau> \<in> T" "s \<in> S" "P s" "t \<in> {0..\<tau>}" "\<forall>\<tau>\<in>{0..t}. G (\<phi> \<tau> s)"
+    and main: "\<forall>s. P s \<longrightarrow> (\<forall>X\<in>Sols (\<lambda>t. f) {0..\<tau>} S 0 s. \<forall>t\<in>{0..\<tau>}. 
+  (\<forall>\<tau>'. 0 \<le> \<tau>' \<and> \<tau>' \<le> \<tau> \<and> \<tau>' \<le> t \<longrightarrow> G (X \<tau>')) \<longrightarrow> Q (X t))"
+  hence "(\<lambda>t. \<phi> t s) \<in> Sols (\<lambda>t. f) {0..\<tau>} S 0 s"
+    using in_ivp_sols_ivl closed_segment_eq_real_ivl[of 0 \<tau>] by force
+  thus "Q (\<phi> t s)"
+    using main hyps by fastforce
+next
+  fix s X t
+  assume hyps: "0 \<le> \<tau>" "\<tau> \<in> T" "P s" "X \<in> Sols (\<lambda>t. f) {0..\<tau>} S 0 s" "t \<in> {0..\<tau>}"  
+    "\<forall>\<tau>'. 0 \<le> \<tau>' \<and> \<tau>' \<le> \<tau> \<and> \<tau>' \<le> t \<longrightarrow> G (X \<tau>')"
+    and main: "\<forall>s\<in>S. P s \<longrightarrow> (\<forall>t\<in>{0..\<tau>}. (\<forall>\<tau>\<in>{0..t}. G (\<phi> \<tau> s)) \<longrightarrow> Q (\<phi> t s))"
+  hence "s \<in> S"
+    using ivp_sols_def[of "\<lambda>t. f"] init_time by auto
+  have obs1: "\<forall>\<tau>\<in>down {0..\<tau>} t. D X = (\<lambda>t. f (X t)) on {0--\<tau>}"
+    apply(clarsimp, rule has_vderiv_on_subset)
+    using ivp_solsD(1)[OF hyps(4)] by (auto simp: closed_segment_eq_real_ivl)
+  have obs2: "X 0 = s" "\<forall>\<tau>\<in>down {0..\<tau>} t. X \<in> {0--\<tau>} \<rightarrow> S"
+    using ivp_solsD(2,3)[OF hyps(4)] by (auto simp: closed_segment_eq_real_ivl)
+  have "\<forall>\<tau>\<in>down {0..\<tau>} t. \<tau> \<in> T"
+  using subintervalI[OF init_time \<open>\<tau> \<in> T\<close>] by (auto simp: closed_segment_eq_real_ivl)
+  hence "\<forall>\<tau>\<in>down {0..\<tau>} t. X \<tau> = \<phi> \<tau> s"
+    using obs1 obs2 apply(clarsimp)
+    by (rule eq_solution_ivl) (auto simp: closed_segment_eq_real_ivl)
+  thus "Q (X t)"
+    using hyps main \<open>s \<in> S\<close> by auto
+qed
+
+lemma sH_orbit: "Hoare \<lceil>P\<rceil> (\<gamma>\<^sup>\<phi>\<^sup>\<bullet>) \<lceil>Q\<rceil> = (\<forall>s \<in> S. P s \<longrightarrow> (\<forall> t \<in> T. Q (\<phi> t s)))"
+  using sH_g_ode unfolding orbit_def g_ode_def by auto
+
+end
+
+\<comment> \<open> Verification with differential invariants \<close>
+
+definition g_ode_inv :: "(('a::banach)\<Rightarrow>'a) \<Rightarrow> 'a pred \<Rightarrow> real set \<Rightarrow> 'a set \<Rightarrow> 
+  real \<Rightarrow> 'a pred \<Rightarrow> 'a nd_fun" ("(1x\<acute>=_ & _ on _ _ @ _ DINV _ )") 
+  where "(x\<acute>= f & G on T S @ t\<^sub>0 DINV I) = (x\<acute>= f & G on T S @ t\<^sub>0)"
+
+lemma sH_g_orbital_guard: 
+  assumes "R = (\<lambda>s. G s \<and> Q s)"
+  shows "Hoare \<lceil>P\<rceil> (x\<acute>= f & G on T S @ t\<^sub>0) \<lceil>Q\<rceil> = Hoare \<lceil>P\<rceil> (x\<acute>= f & G on T S @ t\<^sub>0) \<lceil>R\<rceil>" 
+  using assms unfolding g_orbital_eq ndfun_kat_H ivp_sols_def g_ode_def by auto
+
+lemma sH_g_orbital_inv:
+  assumes "\<lceil>P\<rceil> \<le> \<lceil>I\<rceil>" and "Hoare \<lceil>I\<rceil> (x\<acute>= f & G on T S @ t\<^sub>0) \<lceil>I\<rceil>" and "\<lceil>I\<rceil> \<le> \<lceil>Q\<rceil>"
+  shows "Hoare \<lceil>P\<rceil> (x\<acute>= f & G on T S @ t\<^sub>0) \<lceil>Q\<rceil>"
+  using assms(1) apply(rule_tac p'="\<lceil>I\<rceil>" in H_consl, simp)
+  using assms(3) apply(rule_tac q'="\<lceil>I\<rceil>" in H_consr, simp)
+  using assms(2) by simp
+
+lemma sH_diff_inv[simp]: "Hoare \<lceil>I\<rceil> (x\<acute>= f & G on T S @ t\<^sub>0) \<lceil>I\<rceil> = diff_invariant I f T S t\<^sub>0 G"
+  unfolding diff_invariant_eq ndfun_kat_H g_orbital_eq g_ode_def by auto
+
+lemma H_g_ode_inv: "Hoare \<lceil>I\<rceil> (x\<acute>= f & G on T S @ t\<^sub>0) \<lceil>I\<rceil> \<Longrightarrow> \<lceil>P\<rceil> \<le> \<lceil>I\<rceil> \<Longrightarrow> 
+  \<lceil>\<lambda>s. I s \<and> G s\<rceil> \<le> \<lceil>Q\<rceil> \<Longrightarrow> Hoare \<lceil>P\<rceil> (x\<acute>= f & G on T S @ t\<^sub>0 DINV I) \<lceil>Q\<rceil>"
+  unfolding g_ode_inv_def apply(rule_tac q'="\<lceil>\<lambda>s. I s \<and> G s\<rceil>" in H_consr, simp)
+  apply(subst sH_g_orbital_guard[symmetric], force)
+  by (rule_tac I="I" in sH_g_orbital_inv, simp_all)
+
+
+subsection \<open> Refinement Components \<close>
+
+\<comment> \<open> Skip \<close>
+
+lemma R_skip: "(\<forall>s. P s \<longrightarrow> Q s) \<Longrightarrow> 1 \<le> Ref \<lceil>P\<rceil> \<lceil>Q\<rceil>"
+  by (auto simp: spec_def ndfun_kat_H one_nd_fun_def)
+
+\<comment> \<open> Composition \<close>
+
+lemma R_seq: "(Ref \<lceil>P\<rceil> \<lceil>R\<rceil>) ; (Ref \<lceil>R\<rceil> \<lceil>Q\<rceil>) \<le> Ref \<lceil>P\<rceil> \<lceil>Q\<rceil>"
+  using R_seq by blast
+
+lemma R_seq_rule: "X \<le> Ref \<lceil>P\<rceil> \<lceil>R\<rceil> \<Longrightarrow> Y \<le> Ref \<lceil>R\<rceil> \<lceil>Q\<rceil> \<Longrightarrow> X; Y \<le> Ref \<lceil>P\<rceil> \<lceil>Q\<rceil>"
+  unfolding spec_def by (rule H_seq)
+
+lemmas R_seq_mono = mult_isol_var
+
+\<comment> \<open> Assignment \<close>
+
+lemma R_assign: "(x ::= e) \<le> Ref \<lceil>\<lambda>s. P (\<chi> j. ((($) s)(x := e s)) j)\<rceil> \<lceil>P\<rceil>"
+  unfolding spec_def by (rule H_assign, clarsimp simp: fun_eq_iff fun_upd_def)
+
+lemma R_assign_rule: "(\<forall>s. P s \<longrightarrow> Q (\<chi> j. ((($) s)(x := (e s))) j)) \<Longrightarrow> (x ::= e) \<le> Ref \<lceil>P\<rceil> \<lceil>Q\<rceil>"
+  unfolding sH_assign[symmetric] spec_def .
+
+lemma R_assignl: "P = (\<lambda>s. R (\<chi> j. ((($) s)(x := e s)) j)) \<Longrightarrow> (x ::= e) ; Ref \<lceil>R\<rceil> \<lceil>Q\<rceil> \<le> Ref \<lceil>P\<rceil> \<lceil>Q\<rceil>"
+  apply(rule_tac R=R in R_seq_rule)
+  by (rule_tac R_assign_rule, simp_all)
+
+lemma R_assignr: "R = (\<lambda>s. Q (\<chi> j. ((($) s)(x := e s)) j)) \<Longrightarrow> Ref \<lceil>P\<rceil> \<lceil>R\<rceil>; (x ::= e) \<le> Ref \<lceil>P\<rceil> \<lceil>Q\<rceil>"
+  apply(rule_tac R=R in R_seq_rule, simp)
+  by (rule_tac R_assign_rule, simp)
+
+lemma "(x ::= e) ; Ref \<lceil>Q\<rceil> \<lceil>Q\<rceil> \<le> Ref \<lceil>(\<lambda>s. Q (\<chi> j. ((($) s)(x := e s)) j))\<rceil> \<lceil>Q\<rceil>"
+  by (rule R_assignl) simp
+
+lemma "Ref \<lceil>Q\<rceil> \<lceil>(\<lambda>s. Q (\<chi> j. ((($) s)(x := e s)) j))\<rceil>; (x ::= e) \<le> Ref \<lceil>Q\<rceil> \<lceil>Q\<rceil>"
+  by (rule R_assignr) simp
+
+\<comment> \<open> Conditional \<close>
+
+lemma R_cond: "(IF B THEN Ref \<lceil>\<lambda>s. B s \<and> P s\<rceil> \<lceil>Q\<rceil> ELSE Ref \<lceil>\<lambda>s. \<not> B s \<and> P s\<rceil> \<lceil>Q\<rceil>) \<le> Ref \<lceil>P\<rceil> \<lceil>Q\<rceil>"
+  using R_cond[of "\<lceil>B\<rceil>" "\<lceil>P\<rceil>" "\<lceil>Q\<rceil>"] by simp
+
+lemma R_cond_mono: "X \<le> X' \<Longrightarrow> Y \<le> Y' \<Longrightarrow> (IF P THEN X ELSE Y) \<le> IF P THEN X' ELSE Y'"
+  unfolding kat_cond_def times_nd_fun_def plus_nd_fun_def n_op_nd_fun_def
+  by (auto simp: kcomp_def less_eq_nd_fun_def p2ndf_def le_fun_def)
+
+\<comment> \<open> While loop \<close>
+
+lemma R_while: "WHILE Q INV I DO (Ref \<lceil>\<lambda>s. P s \<and> Q s\<rceil> \<lceil>P\<rceil>) \<le> Ref \<lceil>P\<rceil> \<lceil>\<lambda>s. P s \<and> \<not> Q s\<rceil>"
+  unfolding kat_while_inv_def using R_while[of "\<lceil>Q\<rceil>" "\<lceil>P\<rceil>"] by simp
+
+lemma R_while_mono: "X \<le> X' \<Longrightarrow> (WHILE P INV I DO X) \<le> WHILE P INV I DO X'"
+  by (simp add: kat_while_inv_def kat_while_def mult_isol mult_isor star_iso)
+
+\<comment> \<open> Finite loop \<close>
+
+lemma R_loop: "X \<le> Ref \<lceil>I\<rceil> \<lceil>I\<rceil> \<Longrightarrow> \<lceil>P\<rceil> \<le> \<lceil>I\<rceil> \<Longrightarrow> \<lceil>I\<rceil> \<le> \<lceil>Q\<rceil> \<Longrightarrow> LOOP X INV I \<le> Ref \<lceil>P\<rceil> \<lceil>Q\<rceil>"
+  unfolding spec_def using H_loopI by blast
+
+lemma R_loop_mono: "X \<le> X' \<Longrightarrow> LOOP X INV I \<le> LOOP X' INV I"
+  unfolding kat_loop_inv_def by (simp add: star_iso)
+
+\<comment> \<open> Evolution command (flow) \<close>
+
+lemma R_g_evol: 
+  fixes \<phi> :: "('a::preorder) \<Rightarrow> 'b \<Rightarrow> 'b"
+  shows "(EVOL \<phi> G T) \<le> Ref \<lceil>\<lambda>s. \<forall>t\<in>T. (\<forall>\<tau>\<in>down T t. G (\<phi> \<tau> s)) \<longrightarrow> P (\<phi> t s)\<rceil> \<lceil>P\<rceil>"
+  unfolding spec_def by (rule H_g_evol, simp)
+
+lemma R_g_evol_rule: 
+  fixes \<phi> :: "('a::preorder) \<Rightarrow> 'b \<Rightarrow> 'b"
+  shows "(\<forall>s. P s \<longrightarrow> (\<forall>t\<in>T. (\<forall>\<tau>\<in>down T t. G (\<phi> \<tau> s)) \<longrightarrow> Q (\<phi> t s))) \<Longrightarrow> (EVOL \<phi> G T) \<le> Ref \<lceil>P\<rceil> \<lceil>Q\<rceil>"
+  unfolding sH_g_evol[symmetric] spec_def .
+
+lemma R_g_evoll: 
+  fixes \<phi> :: "('a::preorder) \<Rightarrow> 'b \<Rightarrow> 'b"
+  shows "P = (\<lambda>s. \<forall>t\<in>T. (\<forall>\<tau>\<in>down T t. G (\<phi> \<tau> s)) \<longrightarrow> R (\<phi> t s)) \<Longrightarrow> 
+  (EVOL \<phi> G T) ; Ref \<lceil>R\<rceil> \<lceil>Q\<rceil> \<le> Ref \<lceil>P\<rceil> \<lceil>Q\<rceil>"
+  apply(rule_tac R=R in R_seq_rule)
+  by (rule_tac R_g_evol_rule, simp_all)
+
+lemma R_g_evolr: 
+  fixes \<phi> :: "('a::preorder) \<Rightarrow> 'b \<Rightarrow> 'b"
+  shows "R = (\<lambda>s. \<forall>t\<in>T. (\<forall>\<tau>\<in>down T t. G (\<phi> \<tau> s)) \<longrightarrow> Q (\<phi> t s)) \<Longrightarrow> 
+  Ref \<lceil>P\<rceil> \<lceil>R\<rceil>; (EVOL \<phi> G T) \<le> Ref \<lceil>P\<rceil> \<lceil>Q\<rceil>"
+  apply(rule_tac R=R in R_seq_rule, simp)
+  by (rule_tac R_g_evol_rule, simp)
+
+lemma 
+  fixes \<phi> :: "('a::preorder) \<Rightarrow> 'b \<Rightarrow> 'b"
+  shows "EVOL \<phi> G T ; Ref \<lceil>Q\<rceil> \<lceil>Q\<rceil> \<le> Ref \<lceil>\<lambda>s. \<forall>t\<in>T. (\<forall>\<tau>\<in>down T t. G (\<phi> \<tau> s)) \<longrightarrow> Q (\<phi> t s)\<rceil> \<lceil>Q\<rceil>"
+  by (rule R_g_evoll) simp
+
+lemma 
+  fixes \<phi> :: "('a::preorder) \<Rightarrow> 'b \<Rightarrow> 'b"
+  shows "Ref \<lceil>Q\<rceil> \<lceil>\<lambda>s. \<forall>t\<in>T. (\<forall>\<tau>\<in>down T t. G (\<phi> \<tau> s)) \<longrightarrow> Q (\<phi> t s)\<rceil>; EVOL \<phi> G T \<le> Ref \<lceil>Q\<rceil> \<lceil>Q\<rceil>"
+  by (rule R_g_evolr) simp
+
+\<comment> \<open> Evolution command (ode) \<close>
+
+context local_flow
+begin
+
+lemma R_g_ode: "(x\<acute>= f & G on T S @ 0) \<le> Ref \<lceil>\<lambda>s. s\<in>S \<longrightarrow> (\<forall>t\<in>T. (\<forall>\<tau>\<in>down T t. G (\<phi> \<tau> s)) \<longrightarrow> P (\<phi> t s))\<rceil> \<lceil>P\<rceil>"
+  unfolding spec_def by (rule H_g_ode, simp)
+
+lemma R_g_ode_rule: "(\<forall>s\<in>S. P s \<longrightarrow> (\<forall>t\<in>T. (\<forall>\<tau>\<in>down T t. G (\<phi> \<tau> s)) \<longrightarrow> Q (\<phi> t s))) \<Longrightarrow> 
+  (x\<acute>= f & G on T S @ 0) \<le> Ref \<lceil>P\<rceil> \<lceil>Q\<rceil>"
+  unfolding sH_g_ode[symmetric] by (rule R2)
+
+lemma R_g_odel: "P = (\<lambda>s. \<forall>t\<in>T. (\<forall>\<tau>\<in>down T t. G (\<phi> \<tau> s)) \<longrightarrow> R (\<phi> t s)) \<Longrightarrow> 
+  (x\<acute>= f & G on T S @ 0) ; Ref \<lceil>R\<rceil> \<lceil>Q\<rceil> \<le> Ref \<lceil>P\<rceil> \<lceil>Q\<rceil>"
+  apply(rule_tac R=R in R_seq_rule)
+  by (rule_tac R_g_ode_rule, simp_all)
+
+lemma R_g_oder: "R = (\<lambda>s. \<forall>t\<in>T. (\<forall>\<tau>\<in>down T t. G (\<phi> \<tau> s)) \<longrightarrow> Q (\<phi> t s)) \<Longrightarrow> 
+  Ref \<lceil>P\<rceil> \<lceil>R\<rceil>; (x\<acute>= f & G on T S @ 0) \<le> Ref \<lceil>P\<rceil> \<lceil>Q\<rceil>"
+  apply(rule_tac R=R in R_seq_rule, simp)
+  by (rule_tac R_g_ode_rule, simp)
+
+lemma "(x\<acute>= f & G on T S @ 0) ; Ref \<lceil>Q\<rceil> \<lceil>Q\<rceil> \<le> Ref \<lceil>\<lambda>s. \<forall>t\<in>T. (\<forall>\<tau>\<in>down T t. G (\<phi> \<tau> s)) \<longrightarrow> Q (\<phi> t s)\<rceil> \<lceil>Q\<rceil>"
+  by (rule R_g_odel) simp
+
+lemma "Ref \<lceil>Q\<rceil> \<lceil>\<lambda>s. \<forall>t\<in>T. (\<forall>\<tau>\<in>down T t. G (\<phi> \<tau> s)) \<longrightarrow> Q (\<phi> t s)\<rceil>; (x\<acute>= f & G on T S @ 0) \<le> Ref \<lceil>Q\<rceil> \<lceil>Q\<rceil>"
+  by (rule R_g_oder) simp
+
+lemma R_g_ode_ivl: 
+  "\<tau> \<ge> 0 \<Longrightarrow> \<tau> \<in> T \<Longrightarrow> (\<forall>s\<in>S. P s \<longrightarrow> (\<forall>t\<in>{0..\<tau>}. (\<forall>\<tau>\<in>{0..t}. G (\<phi> \<tau> s)) \<longrightarrow> Q (\<phi> t s))) \<Longrightarrow> 
+  (x\<acute>= f & G on {0..\<tau>} S @ 0) \<le> Ref \<lceil>P\<rceil> \<lceil>Q\<rceil>"
+  unfolding sH_g_ode_ivl[symmetric] by (rule R2)
+
+end
+
+\<comment> \<open> Evolution command (invariants) \<close>
+
+lemma R_g_ode_inv: "diff_invariant I f T S t\<^sub>0 G \<Longrightarrow> \<lceil>P\<rceil> \<le> \<lceil>I\<rceil> \<Longrightarrow> \<lceil>\<lambda>s. I s \<and> G s\<rceil> \<le> \<lceil>Q\<rceil> \<Longrightarrow> 
+  (x\<acute>=f & G on T S @ t\<^sub>0 DINV I) \<le> Ref \<lceil>P\<rceil> \<lceil>Q\<rceil>"
+  unfolding spec_def by (auto simp: H_g_ode_inv)
+
+
+subsection \<open> Derivation of the rules of dL \<close>
+
+text \<open> We derive a generalised version of some domain specific rules of differential dynamic logic (dL).\<close>
+
+lemma diff_solve_axiom: 
+  fixes c::"'a::{heine_borel, banach}"
+  assumes "0 \<in> T" and "is_interval T" "open T"
+    and "\<forall>s. P s \<longrightarrow> (\<forall>t\<in>T. (\<P> (\<lambda> t. s + t *\<^sub>R c) (down T t) \<subseteq> {s. G s}) \<longrightarrow> Q (s + t *\<^sub>R c))"
+  shows "Hoare \<lceil>P\<rceil> (x\<acute>=(\<lambda>s. c) & G on T UNIV @ 0) \<lceil>Q\<rceil>"
+  apply(subst local_flow.sH_g_ode[where f="\<lambda>s. c" and \<phi>="(\<lambda> t x. x + t *\<^sub>R c)"])
+  using line_is_local_flow assms by auto
+
+lemma diff_solve_rule:
+  assumes "local_flow f T UNIV \<phi>"
+    and "\<forall>s. P s \<longrightarrow> (\<forall> t\<in>T. (\<P> (\<lambda>t. \<phi> t s) (down T t) \<subseteq> {s. G s}) \<longrightarrow> Q (\<phi> t s))"
+  shows "Hoare \<lceil>P\<rceil> (x\<acute>= f & G on T UNIV @ 0) \<lceil>Q\<rceil>"
+  using assms by(subst local_flow.sH_g_ode, auto)
+
+lemma diff_weak_rule: 
+  assumes "\<lceil>G\<rceil> \<le> \<lceil>Q\<rceil>"
+  shows "Hoare \<lceil>P\<rceil> (x\<acute>= f & G on T S @ t\<^sub>0) \<lceil>Q\<rceil>"
+  using assms unfolding g_orbital_eq ndfun_kat_H ivp_sols_def g_ode_def by auto
+
+lemma diff_cut_rule:
+  assumes Thyp: "is_interval T" "t\<^sub>0 \<in> T"
+    and wp_C:"Hoare \<lceil>P\<rceil> (x\<acute>= f & G on T S @ t\<^sub>0) \<lceil>C\<rceil>"
+    and wp_Q:"Hoare \<lceil>P\<rceil> (x\<acute>= f & (\<lambda> s. G s \<and> C s) on T S @ t\<^sub>0) \<lceil>Q\<rceil>"
+  shows "Hoare \<lceil>P\<rceil> (x\<acute>= f & G on T S @ t\<^sub>0) \<lceil>Q\<rceil>"
+proof(subst ndfun_kat_H, simp add: g_orbital_eq p2ndf_def g_ode_def, clarsimp)
+  fix t::real and X::"real \<Rightarrow> 'a" and s assume "P s" and "t \<in> T"
+    and x_ivp:"X \<in> ivp_sols (\<lambda>t. f) T S t\<^sub>0 s" 
+    and guard_x:"\<forall>x. x \<in> T \<and> x \<le> t \<longrightarrow> G (X x)"
+  have "\<forall>t\<in>(down T t). X t \<in> g_orbital f G T S t\<^sub>0 s"
+    using g_orbitalI[OF x_ivp] guard_x by auto
+  hence "\<forall>t\<in>(down T t). C (X t)" 
+    using wp_C \<open>P s\<close> by (subst (asm) ndfun_kat_H, auto simp: g_ode_def)
+  hence "X t \<in> g_orbital f (\<lambda>s. G s \<and> C s) T S t\<^sub>0 s"
+    using guard_x \<open>t \<in> T\<close> by (auto intro!: g_orbitalI x_ivp)
+  thus "Q (X t)"
+    using \<open>P s\<close> wp_Q by (subst (asm) ndfun_kat_H) (auto simp: g_ode_def)
+qed
+
+abbreviation g_global_ode ::"(('a::banach)\<Rightarrow>'a) \<Rightarrow> 'a pred \<Rightarrow> 'a nd_fun" ("(1x\<acute>=_ & _)") 
+  where "(x\<acute>= f & G) \<equiv> (x\<acute>= f & G on UNIV UNIV @ 0)"
+
+abbreviation g_global_ode_inv :: "(('a::banach)\<Rightarrow>'a) \<Rightarrow> 'a pred \<Rightarrow> 'a pred \<Rightarrow> 'a nd_fun" 
+  ("(1x\<acute>=_ & _ DINV _)") where "(x\<acute>= f & G DINV I) \<equiv> (x\<acute>= f & G on UNIV UNIV @ 0 DINV I)"
+
+end
