HybridVerifVecs/KAT/kat2rel.thy
@@ -1,36 +1,63 @@
+(*  Title:       Verification and refinement of hybrid systems in the relational KAT
+    Author:      Jonathan Julián Huerta y Munive, 2019
+    Maintainer:  Jonathan Julián Huerta y Munive <jjhuertaymunive1@sheffield.ac.uk>
+*)
+
+section \<open> Verification and refinement of HS in the relational KAT \<close>
+
+text \<open> We use our relational model to obtain verification and refinement components for hybrid 
+programs. We devise three methods for reasoning with evolution commands and their continuous 
+dynamics: providing flows, solutions or invariants. \<close>
+
 theory kat2rel
-  imports
-  "../hs_prelims_dyn_sys"
-  "../../afpModified/VC_KAT"
+  imports 
+    "../hs_prelims_ka"
+    "../hs_prelims_dyn_sys"
 
 begin
 
+subsection \<open> Store and Hoare triples \<close>
 
-chapter\<open> Hybrid System Verification with relations \<close>
+type_synonym 'a pred = "'a \<Rightarrow> bool"
 
 \<comment> \<open>We start by deleting some conflicting notation.\<close>
+
 no_notation Archimedean_Field.ceiling ("\<lceil>_\<rceil>")
         and Archimedean_Field.floor_ceiling_class.floor ("\<lfloor>_\<rfloor>")
-        and Relation.Domain ("r2s")
-        and VC_KAT.gets ("_ ::= _" [70, 65] 61)
         and tau ("\<tau>")
-        and if_then_else_sugar  ("IF _ THEN _ ELSE _ FI" [64,64,64] 63)
+        and proto_near_quantale_class.bres (infixr "\<rightarrow>" 60)
 
 notation Id ("skip")
-     and if_then_else_sugar ("IF _ THEN _ ELSE _" [64,64,64] 63)
 
-section\<open> Verification of regular programs \<close>
+\<comment> \<open>Canonical lifting from predicates to relations and its simplification rules\<close>
 
-text\<open> Below we explore the behavior of the forward box operator from the antidomain kleene algebra
-with the lifting ($\lceil-\rceil$*) operator from predicates to relations @{thm p2r_def[no_vars]} 
-and its dropping counterpart @{thm r2p_def[no_vars]}. \<close>
+definition p2r :: "'a pred \<Rightarrow> 'a rel" ("\<lceil>_\<rceil>") where
+  "\<lceil>P\<rceil> = {(s,s) |s. P s}"
 
-thm sH_H
+lemma p2r_simps[simp]: 
+  "\<lceil>P\<rceil> \<le> \<lceil>Q\<rceil> = (\<forall>s. P s \<longrightarrow> Q s)"
+  "(\<lceil>P\<rceil> = \<lceil>Q\<rceil>) = (\<forall>s. P s = Q s)"
+  "(\<lceil>P\<rceil> ; \<lceil>Q\<rceil>) = \<lceil>\<lambda> s. P s \<and> Q s\<rceil>"
+  "(\<lceil>P\<rceil> \<union> \<lceil>Q\<rceil>) = \<lceil>\<lambda> s. P s \<or> Q s\<rceil>"
+  "rel_tests.t \<lceil>P\<rceil> = \<lceil>P\<rceil>"
+  "(- Id) \<union> \<lceil>P\<rceil> = - \<lceil>\<lambda>s. \<not> P s\<rceil>"
+  "Id \<inter> (- \<lceil>P\<rceil>) = \<lceil>\<lambda>s. \<not> P s\<rceil>"
+  unfolding p2r_def by auto
 
-lemma sH_weaken_pre: "rel_kat.H \<lceil>P2\<rceil> R \<lceil>Q\<rceil> \<Longrightarrow> \<lceil>P1\<rceil> \<subseteq> \<lceil>P2\<rceil> \<Longrightarrow> rel_kat.H \<lceil>P1\<rceil> R \<lceil>Q\<rceil>"
-  unfolding sH_H by auto
+\<comment> \<open> Meaning of the relational hoare triple \<close>
 
-text\<open> Next, we introduce assignments and compute their Hoare triple. \<close>
+lemma rel_kat_H: "rel_kat.Hoare \<lceil>P\<rceil> X \<lceil>Q\<rceil> \<longleftrightarrow> (\<forall>s s'. P s \<longrightarrow> (s,s') \<in> X \<longrightarrow> Q s')"
+  by (simp add: rel_kat.Hoare_def, auto simp add: p2r_def)
+
+\<comment> \<open> Hoare triple for skip and a simp-rule \<close>
+
+lemma H_skip: "rel_kat.Hoare \<lceil>P\<rceil> skip \<lceil>P\<rceil>"
+  using rel_kat.H_skip by blast
+
+lemma sH_skip[simp]: "rel_kat.Hoare \<lceil>P\<rceil> skip \<lceil>Q\<rceil> \<longleftrightarrow> \<lceil>P\<rceil> \<le> \<lceil>Q\<rceil>"
+  unfolding rel_kat_H by simp
+
+\<comment> \<open> We introduce assignments and compute derive their rule of Hoare logic. \<close>
 
 definition vec_upd :: "('a^'b) \<Rightarrow> 'b \<Rightarrow> 'a \<Rightarrow> 'a^'b"
   where "vec_upd s i a \<equiv> (\<chi> j. ((($) s)(i := a)) j)"
@@ -38,98 +65,167 @@ definition vec_upd :: "('a^'b) \<Rightarrow> 'b \<Rightarrow> 'a \<Rightarrow> '
 definition assign :: "'b \<Rightarrow> ('a^'b \<Rightarrow> 'a) \<Rightarrow> ('a^'b) rel" ("(2_ ::= _)" [70, 65] 61) 
   where "(x ::= e) \<equiv> {(s, vec_upd s x (e s))| s. True}" 
 
-lemma sH_assign_iff [simp]: "rel_kat.H \<lceil>P\<rceil> (x ::= e) \<lceil>Q\<rceil> \<longleftrightarrow> (\<forall>s. P s \<longrightarrow> Q (\<chi> j. ((($) s)(x := (e s))) j))"
-  unfolding sH_H vec_upd_def assign_def by (auto simp: fun_upd_def)
+lemma H_assign: "P = (\<lambda>s. Q (\<chi> j. ((($) s)(x := (e s))) j)) \<Longrightarrow> rel_kat.Hoare \<lceil>P\<rceil> (x ::= e) \<lceil>Q\<rceil>"
+  unfolding rel_kat_H assign_def vec_upd_def by force
 
-text\<open> Next, the Hoare rule of the composition:\<close>
+lemma sH_assign[simp]: "rel_kat.Hoare \<lceil>P\<rceil> (x ::= e) \<lceil>Q\<rceil> \<longleftrightarrow> (\<forall>s. P s \<longrightarrow> Q (\<chi> j. ((($) s)(x := (e s))) j))"
+  unfolding rel_kat_H vec_upd_def assign_def by (auto simp: fun_upd_def)
 
-lemma sH_relcomp: "rel_kat.H \<lceil>P\<rceil> X \<lceil>R\<rceil> \<Longrightarrow> rel_kat.H \<lceil>R\<rceil> Y \<lceil>Q\<rceil> \<Longrightarrow> rel_kat.H \<lceil>P\<rceil> (X ; Y) \<lceil>Q\<rceil>"
-  using rel_kat.H_seq_swap by force
+\<comment> \<open> Next, the Hoare rule of the composition \<close>
 
-text\<open> There is also already an implementation of the conditional operator 
-@{thm ifthenelse_def[no_vars]} and its Hoare triple rule: @{thm sH_cond[no_vars]}. \<close>
+lemma H_seq: "rel_kat.Hoare \<lceil>P\<rceil> X \<lceil>R\<rceil> \<Longrightarrow> rel_kat.Hoare \<lceil>R\<rceil> Y \<lceil>Q\<rceil> \<Longrightarrow> rel_kat.Hoare \<lceil>P\<rceil> (X ; Y) \<lceil>Q\<rceil>"
+  by (auto intro: rel_kat.H_seq)
 
-text\<open> Finally, we add a Hoare triple rule for a simple finite iteration. \<close>
+lemma sH_seq: 
+  "rel_kat.Hoare \<lceil>P\<rceil> (X ; Y) \<lceil>Q\<rceil> = rel_kat.Hoare \<lceil>P\<rceil> (X) \<lceil>\<lambda>s. \<forall>s'. (s, s') \<in> Y \<longrightarrow> Q s'\<rceil>"
+  unfolding rel_kat_H by auto
 
-context kat
-begin
+\<comment> \<open> Rewriting the Hoare rule for the conditional statement \<close>
 
-lemma H_star_induct: "H (t i) x i \<Longrightarrow> H (t i) (x\<^sup>\<star>) i"
-  unfolding H_def by (simp add: local.star_sim2)
+abbreviation cond_sugar :: "'a pred \<Rightarrow> 'a rel \<Rightarrow> 'a rel \<Rightarrow> 'a rel" ("IF _ THEN _ ELSE _" [64,64] 63) 
+  where "IF B THEN X ELSE Y \<equiv> rel_kat.kat_cond \<lceil>B\<rceil> X Y"
 
-lemma H_stari: 
-  assumes "t p \<le> t i" and "H (t i) x i" and "t i \<le> t q"
-  shows "H (t p) (x\<^sup>\<star>) q"
-proof-
-  have "H (t i) (x\<^sup>\<star>) i"
-    using assms(2) H_star_induct by blast
-  hence "H (t p) (x\<^sup>\<star>) i"
-    apply(simp add: H_def) 
-    using assms(1) local.phl_cons1 by blast 
-  thus ?thesis 
-    unfolding H_def using assms(3) local.phl_cons2 by blast 
-qed
+lemma H_cond: "rel_kat.Hoare \<lceil>P \<sqinter> B\<rceil> X \<lceil>Q\<rceil> \<Longrightarrow> rel_kat.Hoare \<lceil>P \<sqinter> - B\<rceil> Y \<lceil>Q\<rceil> \<Longrightarrow> 
+  rel_kat.Hoare \<lceil>P\<rceil> (IF B THEN X ELSE Y) \<lceil>Q\<rceil>"
+  by (rule rel_kat.H_cond, auto simp: rel_kat_H)
 
-definition loopi :: "'a \<Rightarrow> 'a \<Rightarrow> 'a" ("loop _ inv _ " [64,64] 63)
-  where "loop x inv i = x\<^sup>\<star>"
+lemma sH_cond[simp]: "rel_kat.Hoare \<lceil>P\<rceil> (IF B THEN X ELSE Y) \<lceil>Q\<rceil> \<longleftrightarrow> 
+  (rel_kat.Hoare \<lceil>P \<sqinter> B\<rceil> X \<lceil>Q\<rceil> \<and> rel_kat.Hoare \<lceil>P \<sqinter> - B\<rceil> Y \<lceil>Q\<rceil>)"
+  by (auto simp: rel_kat.H_cond_iff rel_kat_H)
 
-lemma sH_loopi: "t p \<le> t i \<Longrightarrow> H (t i) x i \<Longrightarrow> t i \<le> t q \<Longrightarrow> H (t p) (loop x inv i) q"
-  unfolding loopi_def using H_stari by blast
+\<comment> \<open> Rewriting the Hoare rule for the while loop \<close>
 
-end
+abbreviation while_inv_sugar :: "'a pred \<Rightarrow> 'a pred \<Rightarrow> 'a rel \<Rightarrow> 'a rel" ("WHILE _ INV _ DO _" [64,64,64] 63) 
+  where "WHILE B INV I DO X \<equiv> rel_kat.kat_while_inv \<lceil>B\<rceil> \<lceil>I\<rceil> X"
+
+lemma sH_while_inv: "\<forall>s. P s \<longrightarrow> I s \<Longrightarrow> \<forall>s. I s \<and> \<not> B s \<longrightarrow> Q s \<Longrightarrow> rel_kat.Hoare \<lceil>I \<sqinter> B\<rceil> X \<lceil>I\<rceil> 
+  \<Longrightarrow> rel_kat.Hoare \<lceil>P\<rceil> (WHILE B INV I DO X) \<lceil>Q\<rceil>"
+  by (rule rel_kat.H_while_inv, auto simp: p2r_def rel_kat.Hoare_def, fastforce)
+
+\<comment> \<open> Finally, we add a Hoare triple rule for finite iterations. \<close>
 
 abbreviation loopi_sugar :: "'a rel \<Rightarrow> 'a pred \<Rightarrow> 'a rel" ("LOOP _ INV _ " [64,64] 63)
-  where "LOOP R INV I \<equiv> rel_kat.loopi R \<lceil>I\<rceil>"
+  where "LOOP X INV I \<equiv> rel_kat.kat_loop_inv X \<lceil>I\<rceil>"
 
-lemma sH_loopI: "\<lceil>P\<rceil> \<subseteq> \<lceil>I\<rceil> \<Longrightarrow> \<lceil>I\<rceil> \<subseteq> \<lceil>Q\<rceil> \<Longrightarrow> rel_kat.H \<lceil>I\<rceil> R \<lceil>I\<rceil> \<Longrightarrow> rel_kat.H \<lceil>P\<rceil> (LOOP R INV I) \<lceil>Q\<rceil>"
-  using rel_kat.sH_loopi[of "\<lceil>P\<rceil>" "\<lceil>I\<rceil>" R "\<lceil>Q\<rceil>"] by auto
+lemma H_loop: "rel_kat.Hoare \<lceil>P\<rceil> X \<lceil>P\<rceil> \<Longrightarrow> rel_kat.Hoare \<lceil>P\<rceil> (LOOP X INV I) \<lceil>P\<rceil>"
+  by (auto intro: rel_kat.H_loop)
+
+lemma H_loopI: "rel_kat.Hoare \<lceil>I\<rceil> X \<lceil>I\<rceil> \<Longrightarrow> \<lceil>P\<rceil> \<subseteq> \<lceil>I\<rceil> \<Longrightarrow> \<lceil>I\<rceil> \<subseteq> \<lceil>Q\<rceil> \<Longrightarrow> rel_kat.Hoare \<lceil>P\<rceil> (LOOP X INV I) \<lceil>Q\<rceil>"
+  using rel_kat.H_loop_inv[of "\<lceil>P\<rceil>" "\<lceil>I\<rceil>" X "\<lceil>Q\<rceil>"] by auto
 
 
-section\<open> Verification of hybrid programs \<close>
+subsection\<open> Verification of hybrid programs \<close>
 
-subsection \<open>Verification by providing evolution\<close>
+\<comment> \<open>Verification by providing evolution\<close>
 
 definition g_evol :: "(('a::ord) \<Rightarrow> 'b \<Rightarrow> 'b) \<Rightarrow> 'b pred \<Rightarrow> 'a set \<Rightarrow> 'b rel" ("EVOL")
   where "EVOL \<phi> G T = {(s,s') |s s'. s' \<in> g_orbit (\<lambda>t. \<phi> t s) G T}"
 
-lemma sH_g_dyn[simp]:  
+lemma H_g_evol: 
   fixes \<phi> :: "('a::preorder) \<Rightarrow> 'b \<Rightarrow> 'b"
-  shows "rel_kat.H \<lceil>P\<rceil> (EVOL \<phi> G T) \<lceil>Q\<rceil> = (\<forall>s. P s \<longrightarrow> (\<forall>t\<in>T. (\<forall>\<tau>\<in>down T t. G (\<phi> \<tau> s)) \<longrightarrow> Q (\<phi> t s)))"
-  unfolding sH_H g_evol_def g_orbit_eq by auto
+  assumes "P = (\<lambda>s. (\<forall>t\<in>T. (\<forall>\<tau>\<in>down T t. G (\<phi> \<tau> s)) \<longrightarrow> Q (\<phi> t s)))"
+  shows "rel_kat.Hoare \<lceil>P\<rceil> (EVOL \<phi> G T) \<lceil>Q\<rceil>"
+  unfolding rel_kat_H g_evol_def g_orbit_eq using assms by clarsimp
 
-subsection \<open>Verification by providing solutions\<close>
+lemma sH_g_evol[simp]:  
+  fixes \<phi> :: "('a::preorder) \<Rightarrow> 'b \<Rightarrow> 'b"
+  shows "rel_kat.Hoare \<lceil>P\<rceil> (EVOL \<phi> G T) \<lceil>Q\<rceil> = (\<forall>s. P s \<longrightarrow> (\<forall>t\<in>T. (\<forall>\<tau>\<in>down T t. G (\<phi> \<tau> s)) \<longrightarrow> Q (\<phi> t s)))"
+  unfolding rel_kat_H g_evol_def g_orbit_eq by auto
+
+\<comment> \<open>Verification by providing solutions\<close>
 
 definition g_ode :: "(('a::banach)\<Rightarrow>'a) \<Rightarrow> 'a pred \<Rightarrow> real set \<Rightarrow> 'a set \<Rightarrow> real \<Rightarrow> 
   'a rel" ("(1x\<acute>=_ & _ on _ _ @ _)") 
   where "(x\<acute>= f & G on T S @ t\<^sub>0) = {(s,s') |s s'. s' \<in> g_orbital f G T S t\<^sub>0 s}"
 
-lemma sH_g_orbital: 
-  "rel_kat.H \<lceil>P\<rceil> (x\<acute>=f & G on T S @ t\<^sub>0) \<lceil>Q\<rceil> = 
+lemma H_g_orbital: 
+  "P = (\<lambda>s. (\<forall>X\<in>ivp_sols (\<lambda>t. f) T S t\<^sub>0 s. \<forall>t\<in>T. (\<forall>\<tau>\<in>down T t. G (X \<tau>)) \<longrightarrow> Q (X t))) \<Longrightarrow> 
+  rel_kat.Hoare \<lceil>P\<rceil> (x\<acute>= f & G on T S @ t\<^sub>0) \<lceil>Q\<rceil>"
+  unfolding rel_kat_H g_ode_def g_orbital_eq by clarsimp
+
+lemma sH_g_orbital: "rel_kat.Hoare \<lceil>P\<rceil> (x\<acute>= f & G on T S @ t\<^sub>0) \<lceil>Q\<rceil> = 
   (\<forall>s. P s \<longrightarrow> (\<forall>X\<in>ivp_sols (\<lambda>t. f) T S t\<^sub>0 s. \<forall>t\<in>T. (\<forall>\<tau>\<in>down T t. G (X \<tau>)) \<longrightarrow> Q (X t)))"
-  unfolding g_orbital_eq g_ode_def image_le_pred sH_H by auto
+  unfolding g_orbital_eq g_ode_def rel_kat_H by auto
 
 context local_flow
 begin
 
-lemma sH_g_orbit: "rel_kat.H \<lceil>P\<rceil> (x\<acute>=f & G on T S @ 0) \<lceil>Q\<rceil> = 
-  (\<forall>s \<in> S. P s \<longrightarrow> (\<forall>t\<in>T. (\<forall>\<tau>\<in>down T t. G (\<phi> \<tau> s)) \<longrightarrow> Q (\<phi> t s)))"
-  unfolding sH_g_orbital apply(clarsimp, safe)
-   apply(erule_tac x=s in allE, simp, erule_tac x="\<lambda>t. \<phi> t s" in ballE)
-  using in_ivp_sols apply(force, force)
-  apply(erule_tac x=s in ballE, simp)
-  apply(subgoal_tac "\<forall>\<tau>\<in>down T t. X \<tau> = \<phi> \<tau> s")
-   apply(simp_all, clarsimp)
-  apply(subst eq_solution, simp_all add: ivp_sols_def)
-  using init_time by auto
+lemma H_g_ode:
+  assumes "P = (\<lambda>s. s \<in> S \<longrightarrow> (\<forall>t\<in>T. (\<forall>\<tau>\<in>down T t. G (\<phi> \<tau> s)) \<longrightarrow> Q (\<phi> t s)))" 
+  shows "rel_kat.Hoare \<lceil>P\<rceil> (x\<acute>= f & G on T S @ 0) \<lceil>Q\<rceil>"
+proof(unfold rel_kat_H g_ode_def g_orbital_eq assms, clarsimp)
+  fix s t X
+  assume hyps: "t \<in> T" "\<forall>x. x \<in> T \<and> x \<le> t \<longrightarrow> G (X x)" "X \<in> Sols (\<lambda>t. f) T S 0 s"
+     and main: "s \<in> S \<longrightarrow> (\<forall>t\<in>T. (\<forall>\<tau>. \<tau> \<in> T \<and> \<tau> \<le> t \<longrightarrow> G (\<phi> \<tau> s)) \<longrightarrow> Q (\<phi> t s))"
+  have "s \<in> S"
+    using ivp_solsD[OF hyps(3)] init_time by auto
+  hence "\<forall>\<tau>\<in>down T t. X \<tau> = \<phi> \<tau> s"
+    using eq_solution hyps by blast
+  thus "Q (X t)"
+    using main \<open>s \<in> S\<close> hyps by fastforce
+qed
+
+lemma sH_g_ode: "rel_kat.Hoare \<lceil>P\<rceil> (x\<acute>= f & G on T S @ 0) \<lceil>Q\<rceil> = 
+  (\<forall>s\<in>S. P s \<longrightarrow> (\<forall>t\<in>T. (\<forall>\<tau>\<in>down T t. G (\<phi> \<tau> s)) \<longrightarrow> Q (\<phi> t s)))"
+proof(unfold sH_g_orbital, clarsimp, safe)
+  fix s t
+  assume hyps: "s \<in> S" "P s" "t\<in>T" "\<forall>\<tau>. \<tau> \<in> T \<and> \<tau> \<le> t \<longrightarrow> G (\<phi> \<tau> s)"
+    and main: "\<forall>s. P s \<longrightarrow> (\<forall>X\<in>Sols (\<lambda>t. f) T S 0 s. \<forall>t\<in>T. (\<forall>\<tau>. \<tau> \<in> T \<and> \<tau> \<le> t \<longrightarrow> G (X \<tau>)) \<longrightarrow> Q (X t))"
+  hence "(\<lambda>t. \<phi> t s) \<in> Sols (\<lambda>t. f) T S 0 s"
+    using in_ivp_sols by blast
+  thus "Q (\<phi> t s)"
+    using main hyps by fastforce
+next
+  fix s X t
+  assume hyps: "P s" "X \<in> Sols (\<lambda>t. f) T S 0 s" "t \<in> T"  "\<forall>\<tau>. \<tau> \<in> T \<and> \<tau> \<le> t \<longrightarrow> G (X \<tau>)"
+    and main: "\<forall>s\<in>S. P s \<longrightarrow> (\<forall>t\<in>T. (\<forall>\<tau>. \<tau> \<in> T \<and> \<tau> \<le> t \<longrightarrow> G (\<phi> \<tau> s)) \<longrightarrow> Q (\<phi> t s))"
+  hence obs: "s \<in> S"
+    using ivp_sols_def[of "\<lambda>t. f"] init_time by auto
+  hence "\<forall>\<tau>\<in>down T t. X \<tau> = \<phi> \<tau> s"
+    using eq_solution hyps by blast
+  thus "Q (X t)"
+    using hyps main obs by auto
+qed
+
+lemma sH_g_ode_ivl: "\<tau> \<ge> 0 \<Longrightarrow> \<tau> \<in> T \<Longrightarrow> rel_kat.Hoare \<lceil>P\<rceil> (x\<acute>= f & G on {0..\<tau>} S @ 0) \<lceil>Q\<rceil> = 
+  (\<forall>s\<in>S. P s \<longrightarrow> (\<forall>t\<in>{0..\<tau>}. (\<forall>\<tau>\<in>{0..t}. G (\<phi> \<tau> s)) \<longrightarrow> Q (\<phi> t s)))"
+proof(unfold sH_g_orbital, clarsimp, safe)
+  fix s t
+  assume hyps: "0 \<le> \<tau>" "\<tau> \<in> T" "s \<in> S" "P s" "t \<in> {0..\<tau>}" "\<forall>\<tau>\<in>{0..t}. G (\<phi> \<tau> s)"
+    and main: "\<forall>s. P s \<longrightarrow> (\<forall>X\<in>Sols (\<lambda>t. f) {0..\<tau>} S 0 s. \<forall>t\<in>{0..\<tau>}. 
+  (\<forall>\<tau>'. 0 \<le> \<tau>' \<and> \<tau>' \<le> \<tau> \<and> \<tau>' \<le> t \<longrightarrow> G (X \<tau>')) \<longrightarrow> Q (X t))"
+  hence "(\<lambda>t. \<phi> t s) \<in> Sols (\<lambda>t. f) {0..\<tau>} S 0 s"
+    using in_ivp_sols_ivl closed_segment_eq_real_ivl[of 0 \<tau>] by force
+  thus "Q (\<phi> t s)"
+    using main hyps by fastforce
+next
+  fix s X t
+  assume hyps: "0 \<le> \<tau>" "\<tau> \<in> T" "P s" "X \<in> Sols (\<lambda>t. f) {0..\<tau>} S 0 s" "t \<in> {0..\<tau>}"  
+    "\<forall>\<tau>'. 0 \<le> \<tau>' \<and> \<tau>' \<le> \<tau> \<and> \<tau>' \<le> t \<longrightarrow> G (X \<tau>')"
+    and main: "\<forall>s\<in>S. P s \<longrightarrow> (\<forall>t\<in>{0..\<tau>}. (\<forall>\<tau>\<in>{0..t}. G (\<phi> \<tau> s)) \<longrightarrow> Q (\<phi> t s))"
+  hence "s \<in> S"
+    using ivp_sols_def[of "\<lambda>t. f"] init_time by auto
+  have obs1: "\<forall>\<tau>\<in>down {0..\<tau>} t. D X = (\<lambda>t. f (X t)) on {0--\<tau>}"
+    apply(clarsimp, rule has_vderiv_on_subset)
+    using ivp_solsD(1)[OF hyps(4)] by (auto simp: closed_segment_eq_real_ivl)
+  have obs2: "X 0 = s" "\<forall>\<tau>\<in>down {0..\<tau>} t. X \<in> {0--\<tau>} \<rightarrow> S"
+    using ivp_solsD(2,3)[OF hyps(4)] by (auto simp: closed_segment_eq_real_ivl)
+  have "\<forall>\<tau>\<in>down {0..\<tau>} t. \<tau> \<in> T"
+  using subintervalI[OF init_time \<open>\<tau> \<in> T\<close>] by (auto simp: closed_segment_eq_real_ivl)
+  hence "\<forall>\<tau>\<in>down {0..\<tau>} t. X \<tau> = \<phi> \<tau> s"
+    using obs1 obs2 apply(clarsimp)
+    by (rule eq_solution_ivl) (auto simp: closed_segment_eq_real_ivl)
+  thus "Q (X t)"
+    using hyps main \<open>s \<in> S\<close> by auto
+qed
 
 lemma sH_orbit: 
-  "rel_kat.H \<lceil>P\<rceil> ({(s,s') | s s'. s' \<in> \<gamma>\<^sup>\<phi> s}) \<lceil>Q\<rceil> = (\<forall>s \<in> S. P s \<longrightarrow> (\<forall> t \<in> T. Q (\<phi> t s)))"
-  using sH_g_orbit unfolding orbit_def g_ode_def by auto
+  "rel_kat.Hoare \<lceil>P\<rceil> ({(s,s') | s s'. s' \<in> \<gamma>\<^sup>\<phi> s}) \<lceil>Q\<rceil> = (\<forall>s \<in> S. P s \<longrightarrow> (\<forall> t \<in> T. Q (\<phi> t s)))"
+  using sH_g_ode unfolding orbit_def g_ode_def by auto
 
 end
 
-
-subsection\<open> Verification with differential invariants \<close>
+\<comment> \<open> Verification with differential invariants \<close>
 
 definition g_ode_inv :: "(('a::banach)\<Rightarrow>'a) \<Rightarrow> 'a pred \<Rightarrow> real set \<Rightarrow> 'a set \<Rightarrow> 
   real \<Rightarrow> 'a pred \<Rightarrow> 'a rel" ("(1x\<acute>=_ & _ on _ _ @ _ DINV _ )") 
@@ -137,67 +233,208 @@ definition g_ode_inv :: "(('a::banach)\<Rightarrow>'a) \<Rightarrow> 'a pred \<R
 
 lemma sH_g_orbital_guard: 
   assumes "R = (\<lambda>s. G s \<and> Q s)"
-  shows "rel_kat.H \<lceil>P\<rceil> (x\<acute>=f & G on T S @ t\<^sub>0) \<lceil>Q\<rceil> = rel_kat.H \<lceil>P\<rceil> (x\<acute>=f & G on T S @ t\<^sub>0) \<lceil>R\<rceil>" 
-  using assms unfolding g_orbital_eq sH_H ivp_sols_def g_ode_def by auto
+  shows "rel_kat.Hoare \<lceil>P\<rceil> (x\<acute>= f & G on T S @ t\<^sub>0) \<lceil>Q\<rceil> = rel_kat.Hoare \<lceil>P\<rceil> (x\<acute>= f & G on T S @ t\<^sub>0) \<lceil>R\<rceil>" 
+  using assms unfolding g_orbital_eq rel_kat_H ivp_sols_def g_ode_def by auto
 
 lemma sH_g_orbital_inv:
-  assumes "\<lceil>P\<rceil> \<le> \<lceil>I\<rceil>" and "rel_kat.H \<lceil>I\<rceil> (x\<acute>=f & G on T S @ t\<^sub>0) \<lceil>I\<rceil>" and "\<lceil>I\<rceil> \<le> \<lceil>Q\<rceil>"
-  shows "rel_kat.H \<lceil>P\<rceil> (x\<acute>=f & G on T S @ t\<^sub>0) \<lceil>Q\<rceil>"
-  using assms(1) apply(rule_tac p'="\<lceil>I\<rceil>" in rel_kat.H_cons_1, simp)
-  using assms(3) apply(rule_tac q'="\<lceil>I\<rceil>" in rel_kat.H_cons_2, simp)
+  assumes "\<lceil>P\<rceil> \<le> \<lceil>I\<rceil>" and "rel_kat.Hoare \<lceil>I\<rceil> (x\<acute>= f & G on T S @ t\<^sub>0) \<lceil>I\<rceil>" and "\<lceil>I\<rceil> \<le> \<lceil>Q\<rceil>"
+  shows "rel_kat.Hoare \<lceil>P\<rceil> (x\<acute>= f & G on T S @ t\<^sub>0) \<lceil>Q\<rceil>"
+  using assms(1) apply(rule_tac p'="\<lceil>I\<rceil>" in rel_kat.H_consl, simp)
+  using assms(3) apply(rule_tac q'="\<lceil>I\<rceil>" in rel_kat.H_consr, simp)
   using assms(2) by simp
 
-lemma sH_diff_inv[simp]: "rel_kat.H \<lceil>I\<rceil> (x\<acute>=f & G on T S @ t\<^sub>0) \<lceil>I\<rceil> = diff_invariant I f T S t\<^sub>0 G"
-  unfolding diff_invariant_eq sH_H g_orbital_eq image_le_pred g_ode_def by auto
+lemma sH_diff_inv[simp]: "rel_kat.Hoare \<lceil>I\<rceil> (x\<acute>= f & G on T S @ t\<^sub>0) \<lceil>I\<rceil> = diff_invariant I f T S t\<^sub>0 G"
+  unfolding diff_invariant_eq rel_kat_H g_orbital_eq g_ode_def by auto
 
-lemma sH_g_odei: "\<lceil>P\<rceil> \<le> \<lceil>I\<rceil> \<Longrightarrow> rel_kat.H \<lceil>I\<rceil> (x\<acute>= f & G on T S @ t\<^sub>0) \<lceil>I\<rceil> \<Longrightarrow> \<lceil>\<lambda>s. I s \<and> G s\<rceil> \<le> \<lceil>Q\<rceil> \<Longrightarrow> 
-  rel_kat.H \<lceil>P\<rceil> (x\<acute>= f & G on T S @ t\<^sub>0 DINV I) \<lceil>Q\<rceil>"
-  unfolding g_ode_inv_def apply(rule_tac q'="\<lceil>\<lambda>s. I s \<and> G s\<rceil>" in rel_kat.H_cons_2, simp)
+lemma H_g_ode_inv: "rel_kat.Hoare \<lceil>I\<rceil> (x\<acute>= f & G on T S @ t\<^sub>0) \<lceil>I\<rceil> \<Longrightarrow> \<lceil>P\<rceil> \<le> \<lceil>I\<rceil> \<Longrightarrow> 
+  \<lceil>\<lambda>s. I s \<and> G s\<rceil> \<le> \<lceil>Q\<rceil> \<Longrightarrow> rel_kat.Hoare \<lceil>P\<rceil> (x\<acute>= f & G on T S @ t\<^sub>0 DINV I) \<lceil>Q\<rceil>"
+  unfolding g_ode_inv_def apply(rule_tac q'="\<lceil>\<lambda>s. I s \<and> G s\<rceil>" in rel_kat.H_consr, simp)
   apply(subst sH_g_orbital_guard[symmetric], force)
   by (rule_tac I="I" in sH_g_orbital_inv, simp_all)
 
-subsection\<open> Derivation of the rules of dL \<close>
 
-text\<open> We derive domain specific rules of differential dynamic logic (dL). In each subsubsection, 
-we first derive the dL axioms (named below with two capital letters and ``D'' being the first one). 
-This is done mainly to prove that there are minimal requirements in Isabelle to get the dL calculus.\<close>
+subsection \<open> Refinement Components \<close>
+
+\<comment> \<open> Skip \<close>
+
+lemma R_skip: "(\<forall>s. P s \<longrightarrow> Q s) \<Longrightarrow> Id \<le> rel_R \<lceil>P\<rceil> \<lceil>Q\<rceil>"
+  by (simp add: rel_rkat.R2 rel_kat_H)
+
+\<comment> \<open> Composition \<close>
+
+lemma R_seq: "(rel_R \<lceil>P\<rceil> \<lceil>R\<rceil>) ; (rel_R \<lceil>R\<rceil> \<lceil>Q\<rceil>) \<le> rel_R \<lceil>P\<rceil> \<lceil>Q\<rceil>"
+  using rel_rkat.R_seq by blast
+
+lemma R_seq_rule: "X \<le> rel_R \<lceil>P\<rceil> \<lceil>R\<rceil> \<Longrightarrow> Y \<le> rel_R \<lceil>R\<rceil> \<lceil>Q\<rceil> \<Longrightarrow> X; Y \<le> rel_R \<lceil>P\<rceil> \<lceil>Q\<rceil>"
+  unfolding rel_rkat.spec_def by (rule H_seq)
+
+lemmas R_seq_mono = relcomp_mono
+
+\<comment> \<open> Assignment \<close>
+
+lemma R_assign: "(x ::= e) \<le> rel_R \<lceil>\<lambda>s. P (\<chi> j. ((($) s)(x := e s)) j)\<rceil> \<lceil>P\<rceil>"
+  unfolding rel_rkat.spec_def by (rule H_assign, clarsimp simp: fun_upd_def)
+
+lemma R_assign_rule: "(\<forall>s. P s \<longrightarrow> Q (\<chi> j. ((($) s)(x := (e s))) j)) \<Longrightarrow> (x ::= e) \<le> rel_R \<lceil>P\<rceil> \<lceil>Q\<rceil>"
+  unfolding sH_assign[symmetric] by (rule rel_rkat.R2)
+
+lemma R_assignl: "P = (\<lambda>s. R (\<chi> j. ((($) s)(x := e s)) j)) \<Longrightarrow> (x ::= e) ; rel_R \<lceil>R\<rceil> \<lceil>Q\<rceil> \<le> rel_R \<lceil>P\<rceil> \<lceil>Q\<rceil>"
+  apply(rule_tac R=R in R_seq_rule)
+  by (rule_tac R_assign_rule, simp_all)
+
+lemma R_assignr: "R = (\<lambda>s. Q (\<chi> j. ((($) s)(x := e s)) j)) \<Longrightarrow> rel_R \<lceil>P\<rceil> \<lceil>R\<rceil>; (x ::= e) \<le> rel_R \<lceil>P\<rceil> \<lceil>Q\<rceil>"
+  apply(rule_tac R=R in R_seq_rule, simp)
+  by (rule_tac R_assign_rule, simp)
+
+lemma "(x ::= e) ; rel_R \<lceil>Q\<rceil> \<lceil>Q\<rceil> \<le> rel_R \<lceil>(\<lambda>s. Q (\<chi> j. ((($) s)(x := e s)) j))\<rceil> \<lceil>Q\<rceil>"
+  by (rule R_assignl) simp
+
+lemma "rel_R \<lceil>Q\<rceil> \<lceil>(\<lambda>s. Q (\<chi> j. ((($) s)(x := e s)) j))\<rceil>; (x ::= e) \<le> rel_R \<lceil>Q\<rceil> \<lceil>Q\<rceil>"
+  by (rule R_assignr) simp
+
+\<comment> \<open> Conditional \<close>
+
+lemma R_cond: "(IF B THEN rel_R \<lceil>\<lambda>s. B s \<and> P s\<rceil> \<lceil>Q\<rceil> ELSE rel_R \<lceil>\<lambda>s. \<not> B s \<and> P s\<rceil> \<lceil>Q\<rceil>) \<le> rel_R \<lceil>P\<rceil> \<lceil>Q\<rceil>"
+  using rel_rkat.R_cond[of "\<lceil>B\<rceil>" "\<lceil>P\<rceil>" "\<lceil>Q\<rceil>"] by simp
+
+lemma R_cond_mono: "X \<le> X' \<Longrightarrow> Y \<le> Y' \<Longrightarrow> (IF P THEN X ELSE Y) \<le> IF P THEN X' ELSE Y'"
+  by (auto simp: rel_kat.kat_cond_def)
+
+\<comment> \<open> While loop \<close>
+
+lemma R_while: "WHILE Q INV I DO (rel_R \<lceil>\<lambda>s. P s \<and> Q s\<rceil> \<lceil>P\<rceil>) \<le> rel_R \<lceil>P\<rceil> \<lceil>\<lambda>s. P s \<and> \<not> Q s\<rceil>"
+  unfolding rel_kat.kat_while_inv_def using rel_rkat.R_while[of "\<lceil>Q\<rceil>" "\<lceil>P\<rceil>"] by simp
+
+lemma R_while_mono: "X \<le> X' \<Longrightarrow> (WHILE P INV I DO X) \<subseteq> WHILE P INV I DO X'"
+  by (simp add: rel_kat.kat_while_inv_def rel_kat.kat_while_def rel_uq.mult_isol 
+      rel_uq.mult_isor rel_ka.star_iso)
+
+\<comment> \<open> Finite loop \<close>
+
+lemma R_loop: "X \<le> rel_R \<lceil>I\<rceil> \<lceil>I\<rceil> \<Longrightarrow> \<lceil>P\<rceil> \<le> \<lceil>I\<rceil> \<Longrightarrow> \<lceil>I\<rceil> \<le> \<lceil>Q\<rceil> \<Longrightarrow> LOOP X INV I \<le> rel_R \<lceil>P\<rceil> \<lceil>Q\<rceil>"
+  unfolding rel_rkat.spec_def using H_loopI by blast
+
+lemma R_loop_mono: "X \<le> X' \<Longrightarrow> LOOP X INV I \<subseteq> LOOP X' INV I"
+  unfolding rel_kat.kat_loop_inv_def by (simp add: rel_ka.star_iso)
+
+\<comment> \<open> Evolution command (flow) \<close>
+
+lemma R_g_evol: 
+  fixes \<phi> :: "('a::preorder) \<Rightarrow> 'b \<Rightarrow> 'b"
+  shows "(EVOL \<phi> G T) \<le> rel_R \<lceil>\<lambda>s. \<forall>t\<in>T. (\<forall>\<tau>\<in>down T t. G (\<phi> \<tau> s)) \<longrightarrow> P (\<phi> t s)\<rceil> \<lceil>P\<rceil>"
+  unfolding rel_rkat.spec_def by (rule H_g_evol, simp)
+
+lemma R_g_evol_rule: 
+  fixes \<phi> :: "('a::preorder) \<Rightarrow> 'b \<Rightarrow> 'b"
+  shows "(\<forall>s. P s \<longrightarrow> (\<forall>t\<in>T. (\<forall>\<tau>\<in>down T t. G (\<phi> \<tau> s)) \<longrightarrow> Q (\<phi> t s))) \<Longrightarrow> (EVOL \<phi> G T) \<le> rel_R \<lceil>P\<rceil> \<lceil>Q\<rceil>"
+  unfolding sH_g_evol[symmetric] rel_rkat.spec_def .
+
+lemma R_g_evoll: 
+  fixes \<phi> :: "('a::preorder) \<Rightarrow> 'b \<Rightarrow> 'b"
+  shows "P = (\<lambda>s. \<forall>t\<in>T. (\<forall>\<tau>\<in>down T t. G (\<phi> \<tau> s)) \<longrightarrow> R (\<phi> t s)) \<Longrightarrow> 
+  (EVOL \<phi> G T) ; rel_R \<lceil>R\<rceil> \<lceil>Q\<rceil> \<le> rel_R \<lceil>P\<rceil> \<lceil>Q\<rceil>"
+  apply(rule_tac R=R in R_seq_rule)
+  by (rule_tac R_g_evol_rule, simp_all)
+
+lemma R_g_evolr: 
+  fixes \<phi> :: "('a::preorder) \<Rightarrow> 'b \<Rightarrow> 'b"
+  shows "R = (\<lambda>s. \<forall>t\<in>T. (\<forall>\<tau>\<in>down T t. G (\<phi> \<tau> s)) \<longrightarrow> Q (\<phi> t s)) \<Longrightarrow> 
+  rel_R \<lceil>P\<rceil> \<lceil>R\<rceil>; (EVOL \<phi> G T) \<le> rel_R \<lceil>P\<rceil> \<lceil>Q\<rceil>"
+  apply(rule_tac R=R in R_seq_rule, simp)
+  by (rule_tac R_g_evol_rule, simp)
+
+lemma 
+  fixes \<phi> :: "('a::preorder) \<Rightarrow> 'b \<Rightarrow> 'b"
+  shows "EVOL \<phi> G T ; rel_R \<lceil>Q\<rceil> \<lceil>Q\<rceil> \<le> rel_R \<lceil>\<lambda>s. \<forall>t\<in>T. (\<forall>\<tau>\<in>down T t. G (\<phi> \<tau> s)) \<longrightarrow> Q (\<phi> t s)\<rceil> \<lceil>Q\<rceil>"
+  by (rule R_g_evoll) simp
+
+lemma 
+  fixes \<phi> :: "('a::preorder) \<Rightarrow> 'b \<Rightarrow> 'b"
+  shows "rel_R \<lceil>Q\<rceil> \<lceil>\<lambda>s. \<forall>t\<in>T. (\<forall>\<tau>\<in>down T t. G (\<phi> \<tau> s)) \<longrightarrow> Q (\<phi> t s)\<rceil>; EVOL \<phi> G T \<le> rel_R \<lceil>Q\<rceil> \<lceil>Q\<rceil>"
+  by (rule R_g_evolr) simp
+
+\<comment> \<open> Evolution command (ode) \<close>
+
+context local_flow
+begin
+
+lemma R_g_ode: "(x\<acute>= f & G on T S @ 0) \<le> rel_R \<lceil>\<lambda>s. s\<in>S \<longrightarrow> (\<forall>t\<in>T. (\<forall>\<tau>\<in>down T t. G (\<phi> \<tau> s)) \<longrightarrow> P (\<phi> t s))\<rceil> \<lceil>P\<rceil>"
+  unfolding rel_rkat.spec_def by (rule H_g_ode, simp)
+
+lemma R_g_ode_rule: "(\<forall>s\<in>S. P s \<longrightarrow> (\<forall>t\<in>T. (\<forall>\<tau>\<in>down T t. G (\<phi> \<tau> s)) \<longrightarrow> Q (\<phi> t s))) \<Longrightarrow> 
+  (x\<acute>= f & G on T S @ 0) \<le> rel_R \<lceil>P\<rceil> \<lceil>Q\<rceil>"
+  unfolding sH_g_ode[symmetric] by (rule rel_rkat.R2)
+
+lemma R_g_odel: "P = (\<lambda>s. \<forall>t\<in>T. (\<forall>\<tau>\<in>down T t. G (\<phi> \<tau> s)) \<longrightarrow> R (\<phi> t s)) \<Longrightarrow> 
+  (x\<acute>= f & G on T S @ 0) ; rel_R \<lceil>R\<rceil> \<lceil>Q\<rceil> \<le> rel_R \<lceil>P\<rceil> \<lceil>Q\<rceil>"
+  apply(rule_tac R=R in R_seq_rule)
+  by (rule_tac R_g_ode_rule, simp_all)
+
+lemma R_g_oder: "R = (\<lambda>s. \<forall>t\<in>T. (\<forall>\<tau>\<in>down T t. G (\<phi> \<tau> s)) \<longrightarrow> Q (\<phi> t s)) \<Longrightarrow> 
+  rel_R \<lceil>P\<rceil> \<lceil>R\<rceil>; (x\<acute>= f & G on T S @ 0) \<le> rel_R \<lceil>P\<rceil> \<lceil>Q\<rceil>"
+  apply(rule_tac R=R in R_seq_rule, simp)
+  by (rule_tac R_g_ode_rule, simp)
+
+lemma "(x\<acute>= f & G on T S @ 0) ; rel_R \<lceil>Q\<rceil> \<lceil>Q\<rceil> \<le> rel_R \<lceil>\<lambda>s. \<forall>t\<in>T. (\<forall>\<tau>\<in>down T t. G (\<phi> \<tau> s)) \<longrightarrow> Q (\<phi> t s)\<rceil> \<lceil>Q\<rceil>"
+  by (rule R_g_odel) simp
+
+lemma "rel_R \<lceil>Q\<rceil> \<lceil>\<lambda>s. \<forall>t\<in>T. (\<forall>\<tau>\<in>down T t. G (\<phi> \<tau> s)) \<longrightarrow> Q (\<phi> t s)\<rceil>; (x\<acute>= f & G on T S @ 0) \<le> rel_R \<lceil>Q\<rceil> \<lceil>Q\<rceil>"
+  by (rule R_g_oder) simp
+
+lemma R_g_ode_ivl: 
+  "\<tau> \<ge> 0 \<Longrightarrow> \<tau> \<in> T \<Longrightarrow> (\<forall>s\<in>S. P s \<longrightarrow> (\<forall>t\<in>{0..\<tau>}. (\<forall>\<tau>\<in>{0..t}. G (\<phi> \<tau> s)) \<longrightarrow> Q (\<phi> t s))) \<Longrightarrow> 
+  (x\<acute>= f & G on {0..\<tau>} S @ 0) \<le> rel_R \<lceil>P\<rceil> \<lceil>Q\<rceil>"
+  unfolding sH_g_ode_ivl[symmetric] by (rule rel_rkat.R2)
+
+end
+
+\<comment> \<open> Evolution command (invariants) \<close>
+
+lemma R_g_ode_inv: "diff_invariant I f T S t\<^sub>0 G \<Longrightarrow> \<lceil>P\<rceil> \<le> \<lceil>I\<rceil> \<Longrightarrow> \<lceil>\<lambda>s. I s \<and> G s\<rceil> \<le> \<lceil>Q\<rceil> \<Longrightarrow> 
+  (x\<acute>=f & G on T S @ t\<^sub>0 DINV I) \<le> rel_R \<lceil>P\<rceil> \<lceil>Q\<rceil>"
+  unfolding rel_rkat.spec_def by (auto simp: H_g_ode_inv)
+
+
+subsection \<open> Derivation of the rules of dL \<close>
+
+text \<open> We derive a generalised version of some domain specific rules of differential dynamic logic (dL).\<close>
 
 lemma diff_solve_axiom: 
   fixes c::"'a::{heine_borel, banach}"
   assumes "0 \<in> T" and "is_interval T" "open T"
     and "\<forall>s. P s \<longrightarrow> (\<forall>t\<in>T. (\<P> (\<lambda> t. s + t *\<^sub>R c) (down T t) \<subseteq> {s. G s}) \<longrightarrow> Q (s + t *\<^sub>R c))"
-  shows "rel_kat.H \<lceil>P\<rceil> (x\<acute>=(\<lambda>s. c) & G on T UNIV @ 0) \<lceil>Q\<rceil>"
-  apply(subst local_flow.sH_g_orbit[where f="\<lambda>s. c" and \<phi>="(\<lambda> t x. x + t *\<^sub>R c)"])
-  using line_is_local_flow assms unfolding image_le_pred by auto
+  shows "rel_kat.Hoare \<lceil>P\<rceil> (x\<acute>=(\<lambda>s. c) & G on T UNIV @ 0) \<lceil>Q\<rceil>"
+  apply(subst local_flow.sH_g_ode[where f="\<lambda>s. c" and \<phi>="(\<lambda> t x. x + t *\<^sub>R c)"])
+  using line_is_local_flow assms by auto
 
 lemma diff_solve_rule:
   assumes "local_flow f T UNIV \<phi>"
     and "\<forall>s. P s \<longrightarrow> (\<forall> t\<in>T. (\<P> (\<lambda>t. \<phi> t s) (down T t) \<subseteq> {s. G s}) \<longrightarrow> Q (\<phi> t s))"
-  shows "rel_kat.H \<lceil>P\<rceil> (x\<acute>=f & G on T UNIV @ 0) \<lceil>Q\<rceil>"
-  using assms by(subst local_flow.sH_g_orbit, auto)
+  shows "rel_kat.Hoare \<lceil>P\<rceil> (x\<acute>= f & G on T UNIV @ 0) \<lceil>Q\<rceil>"
+  using assms by(subst local_flow.sH_g_ode, auto)
 
 lemma diff_weak_rule: 
   assumes "\<lceil>G\<rceil> \<le> \<lceil>Q\<rceil>"
-  shows "rel_kat.H \<lceil>P\<rceil> (x\<acute>=f & G on T S @ t\<^sub>0) \<lceil>Q\<rceil>"
-  using assms unfolding g_orbital_eq sH_H ivp_sols_def g_ode_def by auto
+  shows "rel_kat.Hoare \<lceil>P\<rceil> (x\<acute>= f & G on T S @ t\<^sub>0) \<lceil>Q\<rceil>"
+  using assms unfolding g_orbital_eq rel_kat_H ivp_sols_def g_ode_def by auto
 
 lemma diff_cut_rule:
   assumes Thyp: "is_interval T" "t\<^sub>0 \<in> T"
-    and wp_C:"rel_kat.H \<lceil>P\<rceil> (x\<acute>=f & G on T S @ t\<^sub>0) \<lceil>C\<rceil>"
-    and wp_Q:"rel_kat.H \<lceil>P\<rceil> (x\<acute>=f & (\<lambda> s. G s \<and> C s) on T S @ t\<^sub>0) \<lceil>Q\<rceil>"
-  shows "rel_kat.H \<lceil>P\<rceil> (x\<acute>=f & G on T S @ t\<^sub>0) \<lceil>Q\<rceil>"
-proof(subst sH_H, simp add: g_orbital_eq p2r_def image_le_pred g_ode_def, clarsimp)
+    and wp_C:"rel_kat.Hoare \<lceil>P\<rceil> (x\<acute>= f & G on T S @ t\<^sub>0) \<lceil>C\<rceil>"
+    and wp_Q:"rel_kat.Hoare \<lceil>P\<rceil> (x\<acute>= f & (\<lambda> s. G s \<and> C s) on T S @ t\<^sub>0) \<lceil>Q\<rceil>"
+  shows "rel_kat.Hoare \<lceil>P\<rceil> (x\<acute>= f & G on T S @ t\<^sub>0) \<lceil>Q\<rceil>"
+proof(subst rel_kat_H, simp add: g_orbital_eq p2r_def g_ode_def, clarsimp)
   fix t::real and X::"real \<Rightarrow> 'a" and s assume "P s" and "t \<in> T"
     and x_ivp:"X \<in> ivp_sols (\<lambda>t. f) T S t\<^sub>0 s" 
     and guard_x:"\<forall>x. x \<in> T \<and> x \<le> t \<longrightarrow> G (X x)"
   have "\<forall>t\<in>(down T t). X t \<in> g_orbital f G T S t\<^sub>0 s"
-    using g_orbitalI[OF x_ivp] guard_x unfolding image_le_pred by auto
+    using g_orbitalI[OF x_ivp] guard_x by auto
   hence "\<forall>t\<in>(down T t). C (X t)" 
-    using wp_C \<open>P s\<close> by (subst (asm) sH_H, auto simp: g_ode_def)
+    using wp_C \<open>P s\<close> by (subst (asm) rel_kat_H, auto simp: g_ode_def)
   hence "X t \<in> g_orbital f (\<lambda>s. G s \<and> C s) T S t\<^sub>0 s"
     using guard_x \<open>t \<in> T\<close> by (auto intro!: g_orbitalI x_ivp)
   thus "Q (X t)"
-    using \<open>P s\<close> wp_Q by (subst (asm) sH_H) (auto simp: g_ode_def)
+    using \<open>P s\<close> wp_Q by (subst (asm) rel_kat_H) (auto simp: g_ode_def)
 qed
 
 abbreviation g_global_ode ::"(('a::banach)\<Rightarrow>'a) \<Rightarrow> 'a pred \<Rightarrow> 'a rel" ("(1x\<acute>=_ & _)") 
