ROOT
@@ -5,7 +5,7 @@ session "CPSVerification" = "Ordinary_Differential_Equations" +
     Transformer_Semantics
     KAD
     Algebraic_VCs
-  theories [document = false]
+  (*theories [document = false]
     "afpModified/Antidomain_Semiring"
     "afpModified/Dioid_Models"
     "afpModified/Domain_Semiring"
@@ -19,7 +19,7 @@ session "CPSVerification" = "Ordinary_Differential_Equations" +
     "afpModified/PHL_KAT"
     "afpModified/Range_Semiring"
     "afpModified/VC_KAD"
-    "afpModified/VC_KAT"
+    "afpModified/VC_KAT"*)
   theories
     "HybridVerifVecs/hs_prelims"
     "HybridVerifVecs/hs_prelims_dyn_sys"
@@ -31,8 +31,8 @@ session "CPSVerification" = "Ordinary_Differential_Equations" +
     "HybridVerifVecs/MKA/mka2rel"
     "HybridVerifVecs/MKA/mka2ndfun"
     "HybridVerifVecs/MKA/mka_examples"
-    "HybridVerifVecs/KAT/kat2rel"
     "HybridVerifVecs/KAT/kat2rel_examples"
+    "HybridVerifVecs/KAT/kat2ndfun_examples"
     "HybridVerifLists/VC_diffKAD_auxiliarities"
     "HybridVerifLists/VC_diffKAD"
     "HybridVerifLists/VC_diffKAD_examples"
